Day progress

x86/RealAsm.v
@@ -107,7 +107,27 @@ Section WITHGE.
           step (State rs m) t (State rs' m').
 
 End WITHGE.
-  
+
+  Inductive initial_state_gen (prog: Asm.program) (rs: regset) m: state -> Prop :=
+  | initial_state_gen_intro:
+      forall m1 bstack m2 m3 m4
+        (MALLOC: Mem.alloc (Mem.push_new_stage m) 0 (Mem.stack_limit) = (m1,bstack))
+        (MDROP: Mem.drop_perm m1 bstack 0 (Mem.stack_limit) Writable = Some m2)
+        (MRSB: Mem.record_stack_blocks m2 (make_singleton_frame_adt' bstack frame_info_mono 0) = Some m3)
+        (STORE_RETADDR: Mem.storev Mptr m3 (Vptr bstack (Ptrofs.repr (Mem.stack_limit - size_chunk Mptr))) Vnullptr = Some m4),
+        let ge := Genv.globalenv prog in
+        let rs0 :=
+            rs # PC <- (Genv.symbol_address ge prog.(prog_main) Ptrofs.zero)
+               #RA <- Vnullptr
+               #RSP <- (Val.offset_ptr (Vptr bstack (Ptrofs.repr (Mem.stack_limit))) (Ptrofs.neg (Ptrofs.repr (size_chunk Mptr)))) in
+        initial_state_gen prog rs m (State rs0 m4).
+
+  Inductive initial_state (prog: Asm.program) (rs: regset) (s: state): Prop :=
+  | initial_state_intro: forall m,
+      Genv.init_mem prog = Some m ->
+      initial_state_gen prog rs m s ->
+      initial_state prog rs s.
+
   Definition semantics_gen prog rs m :=
     Semantics step (initial_state_gen prog rs m) final_state (Genv.globalenv prog).
 
