x86/RealAsmproof2.v
@@ -1,0 +1,3388 @@
+Require Import Smallstep.
+Require Import Machregs.
+Require Import Asm.
+Require Import Integers.
+Require Import List.
+Require Import ZArith.
+Require Import Memtype.
+Require Import Memory.
+Require Import Archi.
+Require Import Coqlib.
+Require Import AST.
+Require Import Globalenvs.
+Require Import Events.
+Require Import Values.
+Require Import Conventions1.
+Require Import AsmFacts.
+Require Import RawAsm RealAsm.
+
+Section WITHMEMORYMODEL.
+  
+  Context `{memory_model: Mem.MemoryModel }.
+  Existing Instance inject_perm_upto_writable.
+
+  Context `{external_calls_ops : !ExternalCallsOps mem }.
+  Context `{!EnableBuiltins mem}.
+
+  Existing Instance mem_accessors_default.
+  Existing Instance symbols_inject_instance.
+  Context `{external_calls_props : !ExternalCallsProps mem
+                                    (memory_model_ops := memory_model_ops)
+                                    }.
+
+  Variable prog: Asm.program.
+  Let ge := Genv.globalenv prog.
+  Definition bstack := Genv.genv_next ge.
+  Section PRESERVATION.
+
+  Variable init_stk: stack.
+  Definition init_sp: val := current_sp init_stk.
+  Variable binit_sp: block.
+  Hypothesis init_sp_ptr: init_sp = Vptr binit_sp Ptrofs.zero.
+
+
+  Definition pc_at (s: state): option ((function * instruction) + external_function) :=
+    let '(State rs m) := s in
+    match rs PC with
+    | Vptr b o =>
+      match Genv.find_funct_ptr ge b with
+      | Some (Internal f) =>
+        match find_instr (Ptrofs.unsigned o) (fn_code f) with
+        | Some i => Some (inl (f,i))
+        | None => None
+        end
+      | Some (External ef) => Some (inr ef)
+      | None => None
+      end
+    | _ => None
+    end.
+
+  Definition rs_state s :=
+    let '(State rs _) := s in rs.
+
+  Definition m_state s :=
+    let '(State _ m) := s in m.
+
+  Inductive is_call: instruction -> Prop :=
+  | is_call_s:
+      forall symb b sg,
+        Genv.find_symbol ge symb = Some b ->
+        is_call (Pcall_s symb sg)
+  | is_call_r:
+      forall (r: ireg) sg,
+        is_call (Pcall_r r sg).
+
+  Inductive is_alloc : instruction -> Prop :=
+    is_alloc_intro f sz:
+      is_alloc (Pallocframe f sz).
+
+  Definition make_palloc f : instruction :=
+    let sz := frame_size f in 
+    (Pallocframe f (Ptrofs.sub (Ptrofs.repr (align sz 8)) (Ptrofs.repr (size_chunk Mptr)))).
+
+  Lemma make_palloc_is_alloc:
+    forall f,
+      is_alloc (make_palloc f).
+  Proof. constructor. Qed.
+  
+  Inductive is_free : instruction -> Prop :=
+    is_free_intro sz:
+      is_free (Pfreeframe sz (Ptrofs.sub (Ptrofs.repr sz) (Ptrofs.repr (size_chunk Mptr)))).
+
+  Inductive is_jmp: instruction -> Prop :=
+  | is_jmp_s:
+      forall symb b sg,
+        Genv.find_symbol ge symb = Some b ->
+        is_jmp (Pjmp_s symb sg)
+  | is_jmp_r:
+      forall (r: ireg) sg,
+        is_jmp (Pjmp_r r sg).
+
+  Inductive intermediate_instruction : instruction -> Prop :=
+  | ii_alloc i: is_alloc i -> intermediate_instruction i
+  | ii_jmp i: i = Pret \/ is_jmp i -> intermediate_instruction i.
+
+  Inductive seq: state -> state -> Prop :=
+  | seq_intro rs1 rs2 m (REQ: forall r, rs1 r = rs2 r): seq (State rs1 m) (State rs2 m).
+  
+  Inductive match_states: state -> state -> Prop :=
+  | match_states_call_alloc
+      (rs1 rs2: regset) m1 m2
+      (REQ: forall r : preg, r <> RSP -> rs1 r = rs2 r)
+      (RRSP: rs1 RSP = Val.offset_ptr (rs2 RSP) (Ptrofs.repr (size_chunk Mptr)))
+      (MEQ: Mem.storev Mptr m1 (rs2 RSP) (rs1 RA) = Some m2)
+      f ialloc
+      (PC1: pc_at (State rs1 m1) = Some (inl (f,ialloc)))
+      (ALLOC: is_alloc ialloc):
+      match_states (State rs1 m1) (State rs2 m2)
+  | match_states_call_external
+      (rs1 rs2: regset) m1 m2
+      (REQ: forall r : preg, r <> RSP -> rs1 r = rs2 r)
+      (RRSP: rs1 RSP = Val.offset_ptr (rs2 RSP) (Ptrofs.repr (size_chunk Mptr)))
+      (MEQ: Mem.storev Mptr m1 (rs2 RSP) (rs1 RA) = Some m2)
+      ef
+      (PC1: pc_at (State rs1 m1) = Some (inr ef)):
+      match_states (State rs1 m1) (State rs2 m2)
+  | match_states_free_ret
+      (rs1 rs2: regset) m
+      (REQ: forall r : preg, r <> RSP -> rs1 r = rs2 r)
+      (RRSP: rs1 RSP = Val.offset_ptr (rs2 RSP) (Ptrofs.neg (Ptrofs.repr (size_chunk Mptr))))
+      (LOADRA: exists v, Mem.loadv Mptr m (rs2 RSP) = Some v)
+      f
+      (PC1: pc_at (State rs1 m) = Some (inl (f,Pret))):
+      match_states (State rs1 m) (State rs2 m)
+  | match_states_free_jmp
+      (rs1 rs2: regset) m
+      (REQ: forall r: preg, r <> RSP -> rs1 r = rs2 r)
+      (RRSP: rs1 RSP = Val.offset_ptr (rs2 RSP) (Ptrofs.neg (Ptrofs.repr (size_chunk Mptr))))
+      f ijmp
+      (PC1: pc_at (State rs1 m) = Some (inl (f,ijmp)))
+      (JMP: is_jmp ijmp):
+      match_states (State rs1 m) (State rs2 m)
+  | match_states_normal s1 s2
+                        (SEQ: seq s1 s2)
+                        (PC1: match pc_at s2 with
+                              | Some (inl (f,i)) => ~ intermediate_instruction i
+                              | Some (inr ef) => False
+                              | None => True
+                              end
+                        ):
+      match_states s1 s2.
+
+  Lemma stack_limit_range':
+    size_chunk Mptr <= Mem.stack_limit <= Ptrofs.max_unsigned.
+  Proof.
+    split.
+    generalize Mem.stack_limit_aligned Mem.stack_limit_pos. intros (x & EQ) POS. rewrite EQ.
+    transitivity 8.
+    unfold Mptr. destr; simpl; omega.
+    rewrite EQ in POS. cut (1 <= x). omega.
+    change 0 with (0 * 8) in POS.
+    rewrite <- Z.mul_lt_mono_pos_r in POS. omega. omega.
+    apply Mem.stack_limit_range.
+  Qed.
+
+
+  Lemma nextinstr_nf_pc: forall rs sz, nextinstr_nf rs sz PC = Val.offset_ptr (rs PC) sz.
+  Proof.
+    unfold nextinstr_nf. simpl.
+    intros. rewrite Asmgenproof0.nextinstr_pc. f_equal.
+  Qed.
+
+  Ltac simpl_regs_in H :=
+    repeat first [ rewrite Pregmap.gso in H by congruence
+                 | rewrite Pregmap.gss in H
+                 | rewrite Asmgenproof0.nextinstr_pc in H
+                 | rewrite nextinstr_nf_pc in H
+                 | rewrite Asmgenproof0.nextinstr_inv in H by congruence
+                 ].
+
+  Ltac simpl_regs :=
+    repeat first [ rewrite Pregmap.gso by congruence
+                 | rewrite Pregmap.gss
+                 | rewrite Asmgenproof0.nextinstr_pc
+                 | rewrite nextinstr_nf_pc
+                 | rewrite Asmgenproof0.nextinstr_inv by congruence
+                 ].
+
+  Record wf_asm_function (f: function): Prop :=
+    {
+      wf_asm_call_target_exists:
+        forall o symb sg,
+          find_instr o (fn_code f) = Some (Pcall_s symb sg) ->
+          exists bf f',
+            Genv.symbol_address ge symb Ptrofs.zero = Vptr bf Ptrofs.zero /\
+            Genv.find_funct_ptr ge bf = Some f';
+
+      wf_asm_jmp_target_exists:
+        forall o symb sg,
+          find_instr o (fn_code f) = Some (Pjmp_s symb sg) ->
+          exists bf f',
+            Genv.symbol_address ge symb Ptrofs.zero = Vptr bf Ptrofs.zero /\
+            Genv.find_funct_ptr ge bf = Some f';
+
+      wf_asm_alloc_only_at_beginning:
+        forall o fi ora,
+          find_instr o (fn_code f) = Some (Pallocframe fi ora) ->
+          o = 0;
+      wf_asm_alloc_at_beginning:
+        find_instr 0 (fn_code f) = Some (make_palloc (fn_frame f));
+
+      wf_asm_after_freeframe:
+        forall i o,
+          find_instr (Ptrofs.unsigned o) (fn_code f) = Some i ->
+          is_free i ->
+          exists i' ,
+            find_instr (Ptrofs.unsigned (Ptrofs.add o (Ptrofs.repr (instr_size i)))) (fn_code f) = Some i' /\
+            (i' = Pret \/ is_jmp i' );
+
+      wf_asm_ret_jmp_comes_after_freeframe:
+        forall i o,
+          find_instr (Ptrofs.unsigned o) (fn_code f) = Some i ->
+          i = Pret \/ is_jmp i ->
+          exists o' ifree,
+            find_instr (Ptrofs.unsigned o') (fn_code f) = Some ifree /\
+            is_free ifree /\
+            Ptrofs.unsigned o' + instr_size ifree = Ptrofs.unsigned o;
+
+      wf_asm_pc_repr:
+        forall i o,
+          find_instr (Ptrofs.unsigned o) (fn_code f) = Some i ->
+          Ptrofs.unsigned (Ptrofs.add o (Ptrofs.repr (instr_size i))) = Ptrofs.unsigned o + instr_size i;
+
+      wf_asm_code_bounded:
+        0 <= code_size (fn_code f) <= Ptrofs.max_unsigned;
+
+      wf_asm_builtin_not_PC:
+        forall o ef args res,
+          find_instr o (fn_code f) = Some (Pbuiltin ef args res) ->
+          ~ in_builtin_res res PC;
+
+      wf_asm_jmp_no_rsp:
+        forall o r sg,
+          find_instr o (fn_code f) = Some (Pjmp_r r sg) ->
+          r <> RSP;
+
+      
+    }.
+
+  Lemma wf_asm_wf_allocframe:
+    forall f (WF: wf_asm_function f) o fi ora
+      (FI: find_instr o (fn_code f) = Some (Pallocframe fi ora)),
+      make_palloc (fn_frame f) = Pallocframe fi ora.
+  Proof.
+    intros.
+    exploit wf_asm_alloc_only_at_beginning; eauto. intro; subst.
+    erewrite wf_asm_alloc_at_beginning in FI; eauto. inv FI; auto.
+  Qed.
+    
+  Hypothesis wf_asm_prog:
+    forall b f,
+      Genv.find_funct_ptr ge b = Some (Internal f) ->
+      wf_asm_function f.
+
+  Ltac rewrite_hyps :=
+    repeat
+      match goal with
+        H1 : ?a = _, H2: ?a = _ |- _ => rewrite H1 in H2; inv H2
+      end.
+ 
+  Hypothesis main_internal:
+    exists bmain fmain,
+      Genv.find_symbol ge (prog_main prog) = Some bmain /\
+      Genv.find_funct_ptr ge bmain = Some (Internal fmain).
+  
+  Lemma initial_states_match rs:
+    forall s1 s2,
+      RawAsm.initial_state prog rs s1 ->
+      initial_state prog rs s2 ->
+      exists s1', RawAsm.initial_state prog rs s1' /\ match_states s1' s2.
+  Proof.
+    simpl; intros s1 s2 IS1 IS2.
+    exists s1; split; auto. inv IS1; inv IS2.
+    inv H0; inv H2.
+    destruct main_internal as (bmain & fmain & symbmain & funmain).
+    eapply match_states_call_alloc.
+    - unfold rs0, rs1. intros. simpl_regs. rewrite (Pregmap.gso _ _ H0). auto.
+    - unfold rs0, rs1. simpl_regs. simpl. f_equal. congruence.
+      rewrite Ptrofs.add_assoc. rewrite (Ptrofs.add_commut (Ptrofs.neg _)), Ptrofs.add_neg_zero. rewrite Ptrofs.add_zero. auto.
+    - unfold rs0, rs1; simpl_regs.
+      simpl. rewrite <- Ptrofs.sub_add_opp.
+      unfold Ptrofs.sub.
+      rewrite (Ptrofs.unsigned_repr _ (Mem.stack_limit_range)).
+      rewrite (Ptrofs.unsigned_repr (size_chunk Mptr)).
+      2: vm_compute; intuition congruence.
+      simpl in STORE_RETADDR. congruence.
+    - simpl. unfold rs0. simpl_regs.
+      replace ge0 with ge in * by reflexivity.
+      replace ge1 with ge in * by reflexivity.
+      unfold Genv.symbol_address. rewrite symbmain, funmain.
+      erewrite wf_asm_alloc_at_beginning; eauto.
+    - apply make_palloc_is_alloc.
+  Qed.
+
+  Lemma match_states_PC:
+    forall s1 s2,
+      match_states s1 s2 ->
+      rs_state s1 PC = rs_state s2 PC.
+  Proof.
+    intros s1 s2 MS; inv MS; try rewrite REQ by congruence; try reflexivity.
+    inv SEQ. simpl; auto.
+  Qed.
+
+  Inductive is_builtin: instruction -> Prop :=
+  | is_builtin_intro ef args res: is_builtin (Pbuiltin ef args res).
+
+  Lemma is_builtin_dec i: is_builtin i \/ ~ is_builtin i.
+  Proof.
+    destruct i; first [right; now inversion 1|now econstructor].
+  Qed.
+
+  Lemma step_internal:
+    forall s t s'
+      (STEP: RawAsm.step ge s t s')
+      f i
+      (PCAT: pc_at s = Some (inl (f,i)))
+      (NB: ~ is_builtin i),
+      RawAsm.exec_instr ge f i (rs_state s) (m_state s) = Next (rs_state s') (m_state s') /\ t = E0.
+  Proof.
+    unfold pc_at; intros s t s'  STEP; inv STEP.
+    - rewrite H, H0, H1. inversion 1; subst. simpl. eauto.
+    - rewrite H, H0, H1. intros f0 i A; inv A. intro NIB; exfalso; apply NIB. constructor.
+    - rewrite H, H0. inversion 1.
+  Qed.
+
+  Lemma internal_step:
+    forall rs1 rs2 m1 m2 f i
+      (PCAT: pc_at (State rs1 m1) = Some (inl (f,i)))
+      (EI: RawAsm.exec_instr ge f i rs1 m1 = Next rs2 m2),
+      RawAsm.step ge (State rs1 m1) E0 (State rs2 m2).
+  Proof.
+    intros.
+    simpl in PCAT. repeat destr_in PCAT.
+    eapply RawAsm.exec_step_internal; eauto.
+  Qed.  
+
+  Lemma offset_ptr_neg_sub a b ptr:
+    (Val.offset_ptr (Val.offset_ptr ptr (Ptrofs.neg a)) (Ptrofs.sub a b)) = Val.offset_ptr ptr (Ptrofs.neg b).
+  Proof.
+    rewrite Val.offset_ptr_assoc. f_equal.
+    rewrite Ptrofs.sub_add_opp. rewrite <- Ptrofs.add_assoc.
+    rewrite (Ptrofs.add_commut (Ptrofs.neg _)). rewrite Ptrofs.add_neg_zero. apply Ptrofs.add_zero_l.
+  Qed.
+
+  Lemma offset_ptr_cancel:
+    forall ptr a,
+      (exists b o, ptr = Vptr b o) ->
+      Val.offset_ptr (Val.offset_ptr ptr a) (Ptrofs.neg a) = ptr.
+  Proof.
+    intros ptr a (b & o & EQ); subst. simpl.
+    rewrite <- Ptrofs.sub_add_opp.
+    rewrite Ptrofs.add_commut.
+    rewrite Ptrofs.sub_add_l.
+    rewrite Ptrofs.sub_idem. rewrite Ptrofs.add_zero_l. auto.
+  Qed.
+
+
+  Lemma eval_addrmode_seq:
+    forall (rs rs' : regset) (REQ: forall r, rs r = rs' r) a,
+      eval_addrmode ge a rs = eval_addrmode ge a rs'.
+  Proof.
+    unfold eval_addrmode. intros.
+    destr.
+  Admitted.
+
+  Lemma eval_testcond_seq:
+    forall (rs rs' : regset) (REQ: forall r, rs r = rs' r) t,
+      eval_testcond t rs = eval_testcond t rs'.
+  Proof.
+    unfold eval_testcond. intros.
+    repeat rewrite REQ. repeat destr.
+  Qed.
+  
+  Lemma exec_load_seq:
+    forall chunk m a r r' rd sz r0 m0,
+      seq (State r m) (State r' m) ->
+      exec_load ge chunk m a r rd sz = Next r0 m0 ->
+      exists r1 m1,
+        exec_load ge chunk m a r' rd sz = Next r1 m1.
+  Proof.
+    unfold exec_load; intros chunk m a r r' rd sz r0 m0 SEQ EL; repeat destr_in EL.
+    erewrite eval_addrmode_seq in Heqo. rewrite Heqo. eauto. inv SEQ; auto.
+  Qed.
+
+  Lemma exec_store_seq:
+    forall chunk m a r r' rd lrd sz r0 m0,
+      seq (State r m) (State r' m) ->
+      exec_store ge chunk m a r rd lrd sz = Next r0 m0 ->
+      exists r1 m1,
+        exec_store ge chunk m a r' rd lrd sz = Next r1 m1.
+  Proof.
+    unfold exec_store; intros chunk m a r r' rd lrd sz r0 m0 SEQ EL; repeat destr_in EL.
+    inv SEQ.
+    erewrite eval_addrmode_seq in Heqo. rewrite <- REQ. rewrite Heqo. eauto. auto.
+  Qed.
+
+
+  Lemma nextinstr_eq:
+    forall rs rs',
+      (forall r, rs r = rs' r) ->
+      forall sz r,
+        nextinstr rs sz r = nextinstr rs' sz r.
+  Proof.
+    unfold nextinstr. intros.
+    setoid_rewrite Pregmap.gsspec. destr. apply H.
+  Qed.
+
+  Lemma set_reg_eq:
+    forall (rs rs': regset) r dst,
+      (r <> dst -> rs r = rs' r) ->
+      forall v v' (EQ: v = v'),
+        (rs # dst <- v) r = (rs' # dst <- v') r.
+  Proof.
+    intros.
+    setoid_rewrite Pregmap.gsspec. destr.
+  Qed.
+
+  Lemma undef_regs_eq:
+    forall l (rs rs': regset) r,
+      (~ In r l -> rs r = rs' r) ->
+      undef_regs l rs r = undef_regs l rs' r.
+  Proof.
+    induction l; simpl; intros; eauto.
+    apply IHl. intros; apply set_reg_eq. intros; apply H. intuition. auto.
+  Qed.
+
+  Lemma nextinstr_nf_eq:
+    forall rs rs',
+      (forall r, rs r = rs' r) ->
+      forall sz r,
+        nextinstr_nf rs sz r = nextinstr_nf rs' sz r.
+  Proof.
+    unfold nextinstr_nf. intros.
+    apply nextinstr_eq.
+    intros; apply undef_regs_eq. auto.
+  Qed.
+
+  Lemma set_res_eq:
+    forall res rs rs',
+      (forall r, rs r = rs' r) ->
+      forall r vres,
+        set_res res vres rs r = set_res res vres rs' r.
+  Proof.
+    induction res; simpl; intros; eauto.
+    apply set_reg_eq; auto.
+  Qed.
+
+  Lemma goto_label_seq:
+    forall f l rs1 rs2 m rs' m'
+      (GL : goto_label ge f l rs1 m = Next rs' m')
+      (SEQ: forall r, rs1 r = rs2 r),
+    exists (rs2' : regset) (m2' : mem), goto_label ge f l rs2 m = Next rs2' m2'.
+  Proof.
+    unfold goto_label. intros. destr. rewrite <- SEQ. destr. destr. eauto.
+  Qed.
+  
+  Lemma real_asm_progress rs:
+    forall s1 s2,
+      match_states s1 s2 ->
+      safe (RawAsm.semantics prog rs) s1 ->
+      (exists r : int, final_state s2 r) \/ (exists (t : trace) (s2' : state), step (Genv.globalenv prog) s2 t s2').
+  Proof.
+    intros s1 s2 MS SAFE.
+    destruct (SAFE _  (star_refl _ _ _)) as [(r & FS)|(t & s2' & STEP)].
+    {
+      simpl in FS. inv FS.
+      assert (pc_at (State rs0 m) = None).
+      - simpl. rewrite H. unfold Vnullptr. destruct ptr64; auto.
+      - inv MS; try congruence. inv SEQ.
+        left. eexists; constructor; rewrite <- REQ; eauto.
+    } 
+    simpl in *. fold ge in STEP |- *.
+    inv MS.
+    - exploit step_internal. apply STEP. eauto. intro IB; inv IB; inv ALLOC. intros (EI & T0).
+      simpl in *. subst.
+      inv ALLOC; simpl in EI. repeat destr_in EI.
+      repeat destr_in PC1.
+      exploit wf_asm_wf_allocframe; eauto. intro A; inv A.
+      rewrite offset_ptr_neg_sub in Heqo.
+      rewrite RRSP in Heqo.
+      rewrite offset_ptr_cancel in Heqo.
+      2: unfold Mem.storev in MEQ; destr_in MEQ; eauto.
+      assert (m_state s2' = m2) by congruence. subst.
+      right; do 2 eexists.
+      eapply exec_step_internal.
+      rewrite <- REQ by congruence. eauto. eauto. eauto.
+      simpl. eauto.
+    - admit. (* external call still succeeds after store... *)
+    - exploit step_internal. apply STEP. eauto. intro IB; inv IB. intros (EI & T0).
+      simpl in EI. inv EI.
+      simpl in *.
+      repeat destr_in PC1.
+      destruct LOADRA as (v & LOADRA).
+      right; do 2 eexists.
+      eapply exec_step_internal.
+      rewrite <- REQ by congruence. eauto. eauto. eauto.
+      simpl. rewrite LOADRA. eauto.
+    - exploit step_internal. apply STEP. eauto. intro IB; inv IB; inv JMP. intros (EI & T0).
+      simpl in *.
+      repeat destr_in PC1.
+      inv JMP.
+      + right; do 2 eexists.
+        eapply exec_step_internal.
+        rewrite <- REQ by congruence. eauto. eauto. eauto.
+        simpl in EI; simpl; inv EI. eauto.
+      + right; do 2 eexists.
+        eapply exec_step_internal.
+        rewrite <- REQ by congruence. eauto. eauto. eauto.
+        simpl in EI; repeat destr_in EI. simpl. rewrite <- REQ, Heqo1. eauto.
+        eapply wf_asm_jmp_no_rsp in Heqo0; eauto. congruence.
+    - inversion SEQ; subst.
+      simpl in *. rewrite <- REQ in PC1 by congruence.
+      repeat destr_in PC1; subst.
+      repeat destr_in Heqo.
+      + inv STEP; rewrite_hyps.
+        cut (exists rs2' m2', exec_instr ge f0 i1 rs2 m = Next rs2' m2').
+        intros (rs2' & m2' & EI'). right; exists E0, (State rs2' m2').
+        eapply exec_step_internal. rewrite <- REQ by congruence; eauto. eauto. eauto. eauto.
+        destruct i1; simpl in H6; simpl; eauto using exec_load_seq, exec_store_seq.
+        repeat rewrite <- REQ. repeat destr_in H6. eauto.
+        repeat rewrite <- REQ. repeat destr_in H6. eauto.
+        repeat rewrite <- REQ. repeat destr_in H6. eauto.
+        repeat rewrite <- REQ. repeat destr_in H6. eauto.
+        repeat destr; eauto.
+        eapply goto_label_seq; eauto.
+        rewrite <- REQ; repeat destr_in H6; eauto.
+        erewrite <- eval_testcond_seq by eauto. repeat destr_in H6; eauto using goto_label_seq.
+        erewrite <- eval_testcond_seq by eauto. destr_in H6.
+        erewrite <- eval_testcond_seq by eauto. repeat destr_in H6; eauto using goto_label_seq.
+        rewrite <- REQ. destr. destr. eapply goto_label_seq. eauto. intros.
+        apply set_reg_eq; auto.
+        intros; apply set_reg_eq; auto.
+        inv H6.
+
+
+      assert (PC2: exists i2,
+                 pc_at s2' = Some i2 /\
+                 ((exists f' ialloc, i2 = inl (f',ialloc) /\ is_alloc ialloc )
+                  \/ (exists ef, i2 = inr ef))).
+      {
+        inv JMP.
+        - (* jmp_s*)
+          simpl in EI; repeat destr_in EI.
+          unfold ge in *. rewrite_hyps.
+          unfold pc_at. destruct s2'. simpl in *; subst.
+          simpl_regs.
+          destruct (wf_asm_jmp_target_exists _ (wf_asm_prog _ _ Heqo) _ _ _ Heqo0)
+            as (bf & f' & SA & FFP). 
+          unfold ge in *. rewrite SA.
+          unfold Genv.symbol_address in SA. rewrite H in SA. inv SA. rewrite FFP.
+          destr.
+          + erewrite wf_asm_alloc_at_beginning; eauto.
+            eexists; split; eauto. left; do 2 eexists; split; eauto using make_palloc_is_alloc.
+          + eexists; split; eauto.
+        - simpl in EI.
+          repeat destr_in EI. simpl_regs.
+          unfold pc_at. destruct s2'; simpl in *; subst.
+          unfold Genv.find_funct in Heqo1. repeat destr_in Heqo1.
+          simpl_regs. rewrite H0.
+          destr.
+          erewrite wf_asm_alloc_at_beginning; eauto.
+          eexists; split; eauto. left; do 2 eexists; split; eauto using make_palloc_is_alloc.
+          eexists; split; eauto.
+      }
+      destruct PC2 as (i2 & PC2 & SPEC2).
+      destruct SPEC2 as [(f'  & ialloc & SPEC2 & ALLOC) | (ef & SPEC2)]; subst.
+      right; do 2 eexists.
+      eapply exec_step_internal.
+      rewrite <- REQ by congruence. eauto. eauto. eauto.
+      simpl. rewrite LOADRA. eauto.
+    - 
+
+    
+    destruct (pc_at ge s1) as [[[f i]|ef]|] eqn:PCs.
+    - destruct (is_call_dec i) as [CALL|NOTCALL].
+      + (* it's a call instruction : the next step is going to be either an external function or a Pallocframe. *)
+        simpl in STEP.
+        exploit step_internal; eauto. intro IB; inv IB; inv CALL. intros (EI & T0). subst.
+        destruct (SAFE _ (star_one _ _ _ _ _ STEP)) as [(r & FS)|(t & s3 & STEP2)].
+        * inv FS. simpl in EI.
+          inv CALL; simpl in EI; repeat destr_in EI.
+          -- simpl_regs_in H. unfold Genv.symbol_address in H. repeat destr_in H.
+          -- simpl_regs_in H. rewrite H in Heqo.  inv Heqo.
+        * simpl in STEP2.
+          assert (exists b f', Genv.find_funct_ptr ge b = Some f' /\
+                          rs_state s2 PC = Vptr b Ptrofs.zero).
+          {
+            inv CALL; simpl in EI; repeat destr_in EI.
+            - unfold pc_at in PCs; repeat destr_in PCs; simpl in *; subst.
+              eapply wf_asm_call_target_exists in Heqo0; eauto.
+              destruct Heqo0 as (bf & f' & SA & FFP).
+              inv STEP2; simpl in *; subst; simpl_regs; simpl_regs_in H0; eauto.
+            - simpl_regs. unfold Genv.find_funct in Heqo; repeat destr_in Heqo. eauto.
+          }
+          destruct H as (b & f' & FFP & PC2).
+          inversion STEP2; subst.
+          -- simpl in *. rewrite_hyps.
+             right; exists E0, (State rs' m'). (* split. *)
+             eapply step_call_internal.  5: apply STEP. 5: apply STEP2. eauto.
+             unfold pc_at. rewrite PC2. rewrite H0, H1. eauto. eauto.
+             erewrite wf_asm_alloc_at_beginning in H1; eauto. inv H1. apply make_palloc_is_alloc.
+             (* simpl. *)
+             (* erewrite wf_asm_alloc_at_beginning in H1; eauto. inv H1. *)
+             (* simpl in H2. repeat destr_in H2. unfold ge in FFP; rewrite FFP in H0. inv H0. *)
+             (* simpl_regs. rewrite PC2. simpl. unfold ge. rewrite FFP. *)
+             (* destr. split; inversion 1; subst. intro A. *)
+             (* rewrite Ptrofs.add_zero_l in Heqo0. *)
+             (* inv A. *)
+             (* { *)
+             (*   inv H0. exploit wf_asm_alloc_only_at_beginning. eauto. apply Heqo0. *)
+             (*   rewrite Ptrofs.unsigned_repr by apply instr_size_repr. *)
+             (*   unfold make_palloc. apply not_eq_sym. apply Z.lt_neq. apply instr_size_positive.  *)
+             (* } *)
+             (* { *)
+             (*   exploit wf_asm_ret_jmp_comes_after_freeframe; eauto. *)
+             (*   intros (o' & ifree & FI & IFREE & RNG). *)
+             (*   exploit wf_asm_alloc_at_beginning; eauto. *)
+             (*   intro FALLOC. *)
+             (*   generalize (find_instr_no_overlap' _ _ _ _ _ FI FALLOC). *)
+             (*   rewrite Ptrofs.unsigned_repr in RNG by apply instr_size_repr. *)
+             (*   rewrite RNG. *)
+             (*   intros [EQ|NOOV]. subst; inv IFREE. *)
+             (*   generalize (instr_size_positive (make_palloc (fn_frame f1))) (instr_size_positive ifree). omega. *)
+             (* } *)
+          -- simpl in *. rewrite_hyps.
+             erewrite wf_asm_alloc_at_beginning in H1; eauto. inv H1. 
+          -- simpl in PC2. rewrite_hyps.
+             right; eexists t, (State _ m').
+             eapply step_call_external.  4: apply STEP. 4: apply STEP2. eauto. eauto.
+             unfold pc_at. rewrite PC2. rewrite H0. eauto.
+             Opaque destroyed_at_call.
+             (* simpl. simpl_regs. *)
+             (* unfold pc_at in PCs; repeat destr_in PCs. *)
+             (* assert (rs0 RA = Vptr b (Ptrofs.add i0 (Ptrofs.repr (instr_size i)))). *)
+             (* { *)
+             (*   inv CALL; simpl in EI; repeat destr_in EI; simpl_regs; rewrite Heqv; simpl; auto. *)
+             (* } *)
+             (* rewrite H. rewrite Heqo. destr. split; inversion 1; subst. *)
+             (* intro II; inv II. *)
+             (* { *)
+             (*   inv H4. exploit wf_asm_alloc_only_at_beginning. eauto. apply Heqo1. *)
+             (*   erewrite wf_asm_pc_repr; eauto. *)
+             (*   generalize (Ptrofs.unsigned_range i0) (instr_size_positive i); omega. *)
+             (* } *)
+             (* { *)
+             (*   exploit wf_asm_ret_jmp_comes_after_freeframe; eauto. *)
+             (*   intros (o' & ifree & FI & IFREE & RNG). *)
+             (*   generalize (find_instr_no_overlap _ _ _ _ _ FI Heqo0). *)
+             (*   intro NOOV. trim NOOV. intro EQ; rewrite EQ in FI. rewrite FI in Heqo0; inv Heqo0. inv IFREE; inv CALL. *)
+             (*   erewrite wf_asm_pc_repr in RNG; eauto. rewrite RNG in NOOV.  *)
+             (*   generalize (instr_size_positive ifree) (instr_size_positive i); omega. *)
+             (* } *)
+      + (* not a call, free ? *)
+        destruct (is_free_dec i) as [(sz & ISFREE)|NISFREE].
+        * inversion ISFREE; subst. clear NOTCALL.
+          exploit step_internal; eauto. intro IB; inv IB. intros (EI & T0). subst.
+          assert (PC2: sz = frame_size (fn_frame f) /\ exists i, pc_at ge s2 = Some (inl (f, i)) /\ (i = Pret \/ is_jmp ge i)).
+          {
+            unfold pc_at in PCs |- *. repeat destr_in PCs.
+            destr. simpl in EI. repeat destr_in EI.
+            repeat simpl_regs. rewrite Heqv. simpl. rewrite Heqo.
+            destruct (wf_asm_after_freeframe _ (wf_asm_prog _ _ Heqo) _ _ _ Heqo0 ISFREE) as (SZ & i0 & FI0 & SPECi0). rewrite FI0. eauto. 
+          }
+          destruct PC2 as (SZ & i2 & PC2 & SPECi2). subst.
+          destruct (SAFE _ (star_one _ _ _ _ _ STEP)) as [(r & FS)|(t & s3 & STEP2)].
+          edestruct pc_at_not_final; eauto.
+          simpl in EI. repeat destr_in EI.
+          assert (t = E0).
+          {
+            inv STEP2; auto; unfold ge in *; simpl in *; subst; rewrite_hyps.
+            rewrite H, H2, H3 in PC2. inv PC2. destruct SPECi2 as [A|A]; inv A.
+            rewrite H, H2 in PC2. inv PC2.
+          }
+          subst.
+          destruct SPECi2 as [RET | JMP].
+          -- subst. right.
+             eexists _, _. split. eapply step_free_ret. 4: apply STEP. 4: apply STEP2.
+             eauto. eauto. eauto.
+             exploit step_internal; eauto. intro IB; inv IB. intros (EI & T0).
+             simpl in EI. inv EI. unfold pc_at. destr. simpl in *. subst. simpl_regs.
+             exploit step_internal. apply STEP. eauto. intro IB; inv IB. intros (EI & _).
+             simpl in EI. repeat destr_in EI. simpl_regs. destr. inv Heqo.
+             destr. admit.
+             (* ret should jump right after a call instruction, i.e. not alloc
+             or ret or jmp. (jmp_s and jmp_r are used exclusively for tailcalls,
+             while jmp_l is used for "goto labels") -- not easy to ensure
+             because RA is stored in memory. --> ensure in the semantics ?*)
+          -- exploit step_internal; eauto. intro IB; inv JMP; inv IB. intros (EI & T0).
+             assert (PC3: exists i3,
+                        pc_at ge s3 = Some i3 /\
+                        ((exists f' ialloc, i3 = inl (f',ialloc) /\ is_alloc (frame_size (fn_frame f')) ialloc )
+                         \/ (exists ef, i3 = inr ef))).
+             {
+               unfold pc_at in PC2 |- *. repeat destr_in PC2. destr. simpl in *; subst.
+               inv JMP.
+               - (* jmp_s*)
+                 simpl in EI; repeat destr_in EI.
+                 unfold ge in *. rewrite_hyps.
+                 simpl_regs.
+                 destruct (wf_asm_jmp_target_exists _ (wf_asm_prog _ _ Heqo0) _ _ _ Heqo1)
+                   as (bf & f' & SA & FFP). 
+                 unfold ge in *. rewrite SA.
+                 unfold Genv.symbol_address in SA. rewrite H in SA. inv SA. rewrite FFP.
+                 destr.
+                 erewrite wf_asm_alloc_at_beginning; eauto.
+                 eexists; split; eauto. left; do 2 eexists; split; eauto using make_palloc_is_alloc.
+                 eexists; split; eauto.
+               - simpl in EI.
+                 repeat destr_in EI. simpl_regs.
+                 simpl_regs_in Heqo2.
+                 unfold Genv.find_funct in Heqo2. repeat destr_in Heqo2. rewrite H0.
+                 destr.
+                 erewrite wf_asm_alloc_at_beginning; eauto.
+                 eexists; split; eauto. left; do 2 eexists; split; eauto using make_palloc_is_alloc.
+                 eexists; split; eauto.
+             }
+             destruct PC3 as (i3 & PC3 & SPECi3).
+             destruct (SAFE _ (star_two _ _ _ _ _ _ _ STEP STEP2 eq_refl)) as [(ret & FS)|(t & s4 & STEP3)].
+             edestruct pc_at_not_final; eauto.
+             destruct SPECi3 as [(f' & ialloc & EQ & ALLOC)|(ef&EXT)]; subst.
+             ++
+               edestruct step_internal. apply STEP3. eauto. intro IB; inv IB; inv ALLOC. subst.
+               right; do 2 eexists. split. eapply step_free_tailcall.
+               apply PCs. apply PC2. apply PC3.
+               all: eauto.
+               unfold pc_at in PC3; repeat destr_in PC3.
+               unfold pc_at. destr. subst. simpl in H. inv ALLOC; simpl in H. repeat destr_in H.
+               simpl_regs. rewrite Heqv0. simpl. rewrite Heqo0. repeat destr.
+               intros. split; [intros f1 i1 EQ | intros ef EQ]; inv EQ.
+               intro A; inv A.
+               {
+                 inv H. exploit wf_asm_alloc_only_at_beginning. eauto. apply Heqo3.
+                 erewrite wf_asm_pc_repr; eauto. 
+                 generalize (Ptrofs.unsigned_range i) (instr_size_positive (Pallocframe f0 (Ptrofs.sub (Ptrofs.repr (align (frame_size (fn_frame f1)) 8)) (Ptrofs.repr (size_chunk Mptr)))) ); omega.
+               }
+               {
+                 exploit wf_asm_ret_jmp_comes_after_freeframe; eauto.
+                 intros (o' & ifree & FI & IFREE & RNG).
+                 generalize (find_instr_no_overlap' _ _ _ _ _ FI Heqo1). intros [EQ|NOOV].
+                 destruct H as [H|H]; subst; inv IFREE; inv H.
+                 erewrite wf_asm_pc_repr in RNG; eauto. rewrite <- RNG in NOOV.
+                 generalize (instr_size_positive (Pallocframe f0 (Ptrofs.sub (Ptrofs.repr (align (frame_size (fn_frame f1)) 8)) (Ptrofs.repr (size_chunk Mptr))))).
+                 generalize (instr_size_positive ifree). omega.
+               }
+
+             ++ right; do 2 eexists. split. eapply step_free_external.
+                apply PCs. apply PC2. apply PC3. all: eauto.
+                unfold pc_at in PC3; repeat destr_in PC3.
+                unfold pc_at. destr. subst.
+                inv STEP3; simpl in *; unfold ge in *; rewrite_hyps; try congruence.
+                simpl_regs.
+                assert (r RA = v).
+                edestruct step_internal. apply STEP2. eauto. intro IB; inv IB; inv JMP.
+                edestruct step_internal. apply STEP. eauto. intro IB; inv IB.
+                simpl in H3. rewrite Heqo in H3. inv H3.
+                inv JMP; simpl in H; repeat destr_in H. rewrite <- H6. simpl_regs. auto.
+                rewrite <- H6. simpl_regs. auto.
+                rewrite H.
+                (* ret should jump right after a call instruction, i.e. not alloc
+                   or ret or jmp. (jmp_s and jmp_r are used exclusively for tailcalls,
+                   while jmp_l is used for "goto labels") *)
+                admit.
+
+        * (* not call nor free -> regular step *)
+
+          right; do 2 eexists. split.
+          eapply step_other. eauto.
+          inversion 1; subst. intros f ISFREE; apply NISFREE. eauto.
+          intros. inv H. eapply INV. eauto. 
+          inversion 1; subst; intros; eauto. eauto.
+          destruct (is_builtin_dec i) as [IB|NIB].
+          -- unfold pc_at in PCs; repeat destr_in PCs.
+             simpl in STEP. inv STEP; unfold ge in *; rewrite_hyps; try congruence.
+             inv IB. simpl in H6. congruence.
+             simpl. simpl_regs.
+             rewrite set_res_other.
+             rewrite Asmgenproof0.undef_regs_other.
+             rewrite Heqv. simpl. rewrite Heqo.
+             destr. split;[intros f i0 EQ|intros eef EQ]; inv EQ.
+             intro II; inv II.
+             {
+               inv H. exploit wf_asm_alloc_only_at_beginning. eauto. apply Heqo1.
+               erewrite wf_asm_pc_repr; eauto.
+               generalize (Ptrofs.unsigned_range ofs) (instr_size_positive (Pbuiltin ef args res)); omega.
+             }
+             {
+               exploit wf_asm_ret_jmp_comes_after_freeframe; eauto.
+               intros (o' & ifree & FI & IFREE & RNG).
+               generalize (find_instr_no_overlap _ _ _ _ _ FI Heqo0).
+               intro NOOV. trim NOOV. intro EQ; rewrite EQ in FI. rewrite FI in Heqo0; inv Heqo0. inv IFREE; inv CALL.
+               erewrite wf_asm_pc_repr in RNG; eauto. rewrite RNG in NOOV. 
+               generalize (instr_size_positive ifree) (instr_size_positive (Pbuiltin ef args res)); omega.
+             }
+             {
+               intros r'  IN EQ; subst.
+               apply in_map_iff in IN. destruct IN as (mr & EQ & _).
+               eapply Asmgenproof0.preg_of_not_PC; eauto.
+             }
+             {
+               eapply wf_asm_builtin_not_PC; eauto.
+             }
+          -- edestruct step_internal. apply STEP. eauto. auto. subst.
+             specialize (INV _ _ eq_refl).
+             simpl in *.
+             fold ge in STEP.
+             eapply normal_steps_preserves_normal; eauto.
+
+    - edestruct INV2. eauto.
+    - unfold pc_at in PCs. destr_in PCs. inv STEP; simpl in *; unfold ge in *; repeat destr_in PCs.
+
+  Qed.
+
+  
+  Theorem real_asm_correct rs:
+    backward_simulation (RawAsm.semantics prog rs) (RealAsm.semantics prog rs).
+  Proof.
+    eapply backward_simulation_plus with (match_states := match_states).
+    - reflexivity.
+    - simpl; intros s1 IS1. inv IS1. inv H0.
+      edestruct (Mem.valid_access_store m3 Mptr bstack0 (Mem.stack_limit - size_chunk Mptr) Vnullptr).
+      split;[|split].
+      red; intros. repeat rewrite_perms. rewrite peq_true. split.
+      cut (size_chunk Mptr <=  Mem.stack_limit). omega. apply stack_limit_range'.
+      constructor.
+      apply Z.divide_sub_r. apply Mem.stack_limit_aligned. apply align_size_chunk_divides.
+      intros.
+      red. rewrite_stack_blocks. intro. left. unfold is_stack_top. simpl. auto.
+      eexists; econstructor. eauto. econstructor; eauto. simpl. rewrite Ptrofs.unsigned_repr. eauto.
+      generalize stack_limit_range'. generalize (size_chunk_pos Mptr). omega.
+    - eapply initial_states_match.
+    - simpl; intros s1 s2 r MS FS; inv FS.
+      assert (pc_at s1 = None).
+      {
+        generalize (match_states_PC _ _ MS). intros PCeq.
+        unfold pc_at. destr.  simpl in *. rewrite PCeq.
+        rewrite H. unfold Vnullptr. destruct ptr64; simpl; auto.
+      }
+      inv MS; try congruence.
+      inv SEQ. simpl in *. rewrite REQ in H1. repeat destr_in H1.
+    - simpl.
+  Qed.
+
+
+  Lemma ptrofs_sub_sub a b:
+    Ptrofs.sub (Ptrofs.sub a b) a = Ptrofs.neg b.
+  Proof.
+    rewrite (Ptrofs.sub_add_opp a b).
+    rewrite Ptrofs.sub_add_l. rewrite Ptrofs.sub_idem.
+    apply Ptrofs.add_zero_l.
+  Qed.
+
+  Lemma internal_step:
+    forall s f i
+      (PCAT: pc_at ge s = Some (inl (f,i)))
+      (NB: ~ is_builtin i) rs' m'
+      (EI: exec_instr ge f i (rs_state s) (m_state s) = Next rs' m'),
+      RealAsm.step ge s E0 (State rs' m').
+  Proof.
+    unfold pc_at; intros s f i PCAT NB rs' m' EI.
+    repeat destr_in PCAT.
+    eapply RealAsm.exec_step_internal; eauto.
+  Qed.
+
+  Ltac force_rewrite_match H :=
+    match goal with
+      H: ?b = _ |- context [ match ?a with _ => _ end ] =>
+      cut (b = a);[ let A := fresh in intro A; rewrite <- A, H | ]
+    end.
+  Ltac simpl_regs_in H :=
+    repeat first [ rewrite Pregmap.gso in H by congruence
+                 | rewrite Pregmap.gss in H
+                 | rewrite Asmgenproof0.nextinstr_pc in H
+                 | rewrite nextinstr_nf_pc in H
+                 | rewrite Asmgenproof0.nextinstr_inv in H by congruence
+                 ].
+
+  Ltac simpl_regs :=
+    repeat first [ rewrite Pregmap.gso by congruence
+                 | rewrite Pregmap.gss
+                 | rewrite Asmgenproof0.nextinstr_pc
+                 | rewrite nextinstr_nf_pc
+                 | rewrite Asmgenproof0.nextinstr_inv by congruence
+                 ].
+
+  Lemma nextinstr_eq:
+    forall rs rs',
+      (forall r, rs r = rs' r) ->
+      forall sz r,
+        nextinstr rs sz r = nextinstr rs' sz r.
+  Proof.
+    unfold nextinstr. intros.
+    setoid_rewrite Pregmap.gsspec. destr. apply H.
+  Qed.
+
+  Lemma set_reg_eq:
+    forall (rs rs': regset) r dst,
+      (r <> dst -> rs r = rs' r) ->
+      forall v v' (EQ: v = v'),
+        (rs # dst <- v) r = (rs' # dst <- v') r.
+  Proof.
+    intros.
+    setoid_rewrite Pregmap.gsspec. destr.
+  Qed.
+
+  Lemma undef_regs_eq:
+    forall l (rs rs': regset) r,
+      (~ In r l -> rs r = rs' r) ->
+      undef_regs l rs r = undef_regs l rs' r.
+  Proof.
+    induction l; simpl; intros; eauto.
+    apply IHl. intros; apply set_reg_eq. intros; apply H. intuition. auto.
+  Qed.
+
+  Lemma nextinstr_nf_eq:
+    forall rs rs',
+      (forall r, rs r = rs' r) ->
+      forall sz r,
+        nextinstr_nf rs sz r = nextinstr_nf rs' sz r.
+  Proof.
+    unfold nextinstr_nf. intros.
+    apply nextinstr_eq.
+    intros; apply undef_regs_eq. auto.
+  Qed.
+
+  Lemma set_res_eq:
+    forall res rs rs',
+      (forall r, rs r = rs' r) ->
+      forall r vres,
+        set_res res vres rs r = set_res res vres rs' r.
+  Proof.
+    induction res; simpl; intros; eauto.
+    apply set_reg_eq; auto.
+  Qed.
+
+  Axiom frame_size_aligned:
+    forall f,
+      frame_size f = align (frame_size f) 8.
+
+  
+  Lemma steps_correct:
+    forall s1 t s2
+      (STEP : step (Genv.globalenv prog) s1 t s2)
+    s1' (SEQ: seq s1 s1'),
+    exists s2',
+      plus RealAsm.step (Genv.globalenv prog) s1' t s2'
+      /\ seq s2 s2'.
+  Proof.
+    intros s1 t s2 STEP s1' SEQ; inv STEP.
+    - (* call -> alloc *)
+      inv SEQ.
+      edestruct (step_internal _ _ _ _ STEP1) as (EI1 & T1); eauto. intro IB; inv IB; inv CALL.
+      edestruct (step_internal _ _ _ _ STEP2) as (EI2 & T2); eauto. intro IB; inv IB; inv ALLOC.
+      inv ALLOC. simpl in EI2; repeat destr_in EI2.
+      destruct s2, s3; simpl in *. subst.
+
+      assert (call_ok: m1 = m /\ exists b rs',
+                  r0 PC = Vptr b Ptrofs.zero /\ Genv.find_funct_ptr ge b = Some (Internal f) /\
+                  exec_instr ge f0 icall rs2 m = Next rs' m0 /\
+                  (forall r:preg, r <> RSP -> rs' r = r0 r) /\
+                  rs' RSP = Val.offset_ptr (rs2 RSP) (Ptrofs.neg (Ptrofs.repr (size_chunk Mptr))) /\
+                  r0 RSP = rs1 RSP).
+      {
+        unfold pc_at in PC2. repeat destr_in PC2.
+        split.
+        inv CALL; simpl in EI1; repeat destr_in EI1; eauto.
+        exists b.
+        inv CALL; simpl in EI1; repeat destr_in EI1.
+        - simpl_regs_in Heqv. revert Heqv.  unfold Genv.symbol_address. rewrite H0. intro A; inv A.
+          unfold ge. rewrite Heqo0.
+          simpl.
+          force_rewrite_match Heqo.
+          + eexists; repeat apply conj; eauto.
+            * intros. rewrite (Pregmap.gso _ _ H2).
+              simpl_regs. unfold Genv.symbol_address. unfold ge. rewrite H0. rewrite REQ.
+              apply set_reg_eq. intros.
+              apply set_reg_eq. auto.
+              auto. auto.
+          + rewrite ! REQ.
+            f_equal.
+            simpl_regs. 
+            rewrite Val.offset_ptr_assoc.
+            rewrite Ptrofs.add_commut.
+            rewrite <- Ptrofs.sub_add_opp.
+            rewrite H, ptrofs_sub_sub. rewrite REQ. auto.
+        - simpl_regs_in Heqv. revert Heqv. rewrite H0. intro A; inv A.
+          unfold ge. rewrite Heqo0.
+          simpl.
+          force_rewrite_match Heqo.
+          + eexists; repeat apply conj; eauto.
+            * intros. rewrite (Pregmap.gso _ _ H2).
+              simpl_regs.
+              apply set_reg_eq; auto. intros.
+              apply set_reg_eq. auto. rewrite REQ. auto.
+              rewrite <- REQ. auto.
+          + rewrite ! REQ.
+            f_equal.
+            simpl_regs. 
+            rewrite Val.offset_ptr_assoc.
+            rewrite Ptrofs.add_commut.
+            rewrite <- Ptrofs.sub_add_opp.
+            rewrite H, ptrofs_sub_sub. rewrite REQ. auto.
+      }
+      destruct call_ok as (MEQ & b & rs' & PC3 & FFP & EIcall & SAMErs & rs'RSP & r0RSP).
+      subst.
+      eexists; split. eapply plus_two.
+      eapply internal_step; eauto.
+      rewrite <- PC1.
+      unfold ge. simpl. rewrite <- REQ. auto. intro IB; inv IB; inv CALL.
+      eapply internal_step; eauto.
+      rewrite <- PC2. rewrite <- SAMErs by congruence.
+      unfold ge. simpl. auto.
+      inversion 1.
+      simpl. eauto. traceEq.
+      econstructor.
+      apply nextinstr_eq.
+      intros. apply set_reg_eq; auto.
+      intros. rewrite rs'RSP.
+      apply set_reg_eq; auto. intros. rewrite <- SAMErs; eauto.
+      rewrite r0RSP.
+      rewrite REQ.
+      rewrite Val.offset_ptr_assoc. rewrite Ptrofs.add_commut.
+      rewrite Ptrofs.add_neg_zero.
+      admit. (* RSP should be a pointer *)
+      rewrite r0RSP. rewrite rs'RSP. rewrite REQ.
+      rewrite Val.offset_ptr_assoc. f_equal.
+      rewrite <- Ptrofs.neg_add_distr. f_equal.
+      rewrite Ptrofs.sub_add_opp.
+      rewrite (Ptrofs.add_commut _ (Ptrofs.neg _)).
+      rewrite <- Ptrofs.add_assoc. rewrite Ptrofs.add_neg_zero. rewrite Ptrofs.add_zero_l; auto.
+    - admit.                    (* call -> external *)
+    - (* free -> ret *)
+      inv SEQ.
+      edestruct (step_internal _ _ _ _ STEP1) as (EI1 & T1); eauto. intro IB; inv IB; inv FREE.
+      edestruct (step_internal _ _ _ _ STEP2) as (EI2 & T2); eauto. intro IB; inv IB.
+      inv FREE. simpl in EI1; repeat destr_in EI1.
+      simpl in EI2. inv EI2.
+      destruct s2, s3; simpl in *. subst.
+      simpl_regs_in PC2.
+      repeat destr_in PC1. simpl in PC2.
+      repeat destr_in PC2.
+      eexists. split.
+      eapply plus_two.
+      eapply internal_step. simpl.
+      unfold ge. rewrite <- REQ, Heqv0, Heqo2, Heqo1. eauto.
+      inversion 1.
+      simpl. eauto.
+      eapply internal_step. simpl. simpl_regs.
+      unfold ge. rewrite <- REQ, Heqv0. simpl.
+      rewrite Heqo2, Heqo3. eauto. inversion 1.
+      simpl. force_rewrite_match Heqo. eauto.
+      f_equal. simpl_regs.
+      rewrite REQ. f_equal.
+      rewrite Z.max_r by apply frame_size_pos. rewrite <- frame_size_aligned. auto.
+      traceEq.
+      constructor. intros.
+      simpl_regs.
+      apply set_reg_eq.
+      intros; apply set_reg_eq.
+      intros.
+      repeat simpl_regs.
+      intros; apply set_reg_eq.
+      intros. simpl_regs. auto.
+      rewrite Val.offset_ptr_assoc. f_equal. auto.
+      rewrite <- Ptrofs.sub_add_l.
+      rewrite Ptrofs.add_commut.
+      rewrite Ptrofs.sub_add_l.
+      rewrite Ptrofs.sub_idem. rewrite Ptrofs.add_zero_l. auto. auto. auto.
+    - admit. (* free -> jmp -> alloc (tailcall to internal function) *)
+    - admit. (* free -> jmp -> external (tailcall to external function) *)
+    - (* regular instruction *)
+      inv STEP0; simpl in PC; rewrite H in PC; repeat destr_in PC; inv H0.
+      rewrite Heqo0 in H1; inv H1.
+      inv SEQ.
+      eexists; split. apply plus_one.
+      eapply RealAsm.exec_step_internal. rewrite <- REQ; eauto. eauto. eauto.
+
+      Lemma exec_instr_same_rs:
+        forall f i rs m rs' m' rs2 (SEQ: seq (State rs m) (State rs2 m))
+          (EI: RawAsm.exec_instr ge f i rs m = Next rs' m'),
+        exists rs2',
+          exec_instr ge f i rs2 m = Next rs2' m' /\ seq (State rs' m') (State rs2' m').
+      Proof.
+        
+      Qed.
+
+      eapply
+      
+  Qed.
+
+  Theorem real_asm_correct rs:
+    forward_simulation (RawAsmMergeSteps.semantics prog rs) (RealAsm.semantics prog rs).
+  Proof.
+    eapply forward_simulation_plus with (match_states := fun s1 s2 : Asm.state => s1 = s2).
+    - reflexivity.
+    - intros; eauto.
+    - intros; subst; eauto.
+    - simpl. intros; subst.
+      eexists; split; eauto.
+      
+      inv H.
+      + eapply plus_two; eauto.
+      inv H; first [ eapply plus_one; eauto; try reflexivity
+                   | eapply plus_two; eauto; try reflexivity
+                   | eapply plus_three; eauto; try reflexivity ].
+  Qed.
+
+  
+
+  Ltac rewrite_hyps :=
+    repeat
+      match goal with
+        H1 : ?a = _, H2: ?a = _ |- _ => rewrite H1 in H2; inv H2
+      end.
+
+  Ltac simpl_regs_in H :=
+    repeat rewrite Pregmap.gso in H by congruence;
+    try rewrite Pregmap.gss in H.
+
+  Ltac simpl_regs :=
+    repeat rewrite Pregmap.gso by congruence;
+    try rewrite Pregmap.gss.
+
+  Definition measure (s: state) : nat :=
+    match classify_state_bool s with
+    | Some SKcall => 2%nat
+    | Some SKret => 0%nat
+    | _ => 1%nat
+    end.
+
+  Lemma instr_size_not_zero:
+    forall i,
+      instr_size i <> 0.
+  Proof.
+    intros; apply not_eq_sym; apply Z.lt_neq, instr_size_positive.
+  Qed.
+
+  Lemma eval_builtin_arg_eq_rs:
+    forall (rs1 rs2: regset) (REQ: forall r, rs1 r = rs2 r) sp m args vargs,
+      eval_builtin_arg ge rs1 sp m args vargs ->
+      eval_builtin_arg ge rs2 sp m args vargs.
+  Proof.
+    induction 2; rewrite ? REQ; econstructor; eauto.
+  Qed.
+
+  Lemma eval_builtin_args_eq_rs:
+    forall (rs1 rs2: regset) (REQ: forall r, rs1 r = rs2 r) sp m args vargs,
+      eval_builtin_args ge rs1 sp m args vargs ->
+      eval_builtin_args ge rs2 sp m args vargs.
+  Proof.
+    induction 2; constructor; eauto using eval_builtin_arg_eq_rs.
+  Qed.
+
+  Fixpoint in_builtin_res (b: builtin_res preg) (r:preg) :=
+    match b with
+    | BR b => b = r
+    | BR_none => False
+    | BR_splitlong hi lo => in_builtin_res hi r \/ in_builtin_res lo r
+    end.
+
+  Lemma set_res_other:
+    forall res vres rs r,
+      ~ in_builtin_res res r ->
+      set_res res vres rs r = rs r.
+  Proof.
+    induction res; simpl; intros; eauto.
+    rewrite Pregmap.gso; auto.
+    rewrite IHres2. apply IHres1. intuition. intuition.
+  Qed.
+
+  Theorem real_step_correct:
+    forall s1 t s1' (STEP: RawAsm.step ge s1 t s1')
+      s2 (MS: match_states s1 s2),
+   (exists s2', plus RealAsm.step ge s2 t s2' /\ match_states s1' s2') \/
+   (measure s1' < measure s1)%nat /\ t = E0 /\ match_states s1' s2.
+  Proof.
+    intros s1 t s1' STEP s2 MS.
+    inv MS.
+    - inv STEP.
+      + (* internal *)
+        destruct (instr_same i) eqn:SAME.
+        admit.
+        destruct i; simpl in SAME; try congruence.
+        * (* call_s *)
+          simpl. simpl in H2. inv H2.
+          right.
+          destruct (calls_to_defined_functions _ _ _ _ _ H0 H1) as (bf & f' & SA & FFP).
+          rewrite SA.
+          assert (FS: Genv.find_symbol ge symb = Some bf).
+          {
+            unfold Genv.symbol_address in SA; repeat destr_in SA.
+          }
+          split.
+          -- unfold measure. unfold classify_state_bool.
+             rewrite H, H0, H1. simpl.
+             rewrite FFP. rewrite FS. destr. 2: omega.
+             destr_in Heqo.
+             erewrite pallocframe_at_beginning in Heqo; eauto. simpl in Heqo. inv Heqo. omega.
+             inv Heqo. omega.
+          -- split; auto.
+             eapply match_states_call.
+             3: eapply RawAsm.exec_step_internal.
+             3: apply H. eauto. econstructor; eauto. econstructor; eauto. eauto. eauto.
+             simpl. f_equal. rewrite SA. reflexivity.
+        * (* call_r *) admit.
+        * (* ret *)
+          specialize (CL SKret).
+          edestruct CL; [|congruence].
+          repeat econstructor; eauto.
+        * (* allocframe *)
+          specialize (CL SKalloc).
+          edestruct CL; [|congruence].
+          repeat econstructor; eauto.
+        * (* freeframe *)
+          destruct (after_freeframe _ _ _ _ _ H0 H1) as (i & NEXTINSTR & CHOICES).
+          destruct CHOICES.
+          {
+            right.
+            split.
+            - simpl in H2. repeat destr_in H2.
+              unfold measure, classify_state_bool. rewrite Asmgenproof0.nextinstr_pc. simpl_regs.
+              rewrite H. simpl. rewrite H0, H1. rewrite NEXTINSTR.
+              simpl. omega.
+            - split; auto.
+              eapply match_states_freeframe; eauto.
+              2: eapply RawAsm.exec_step_internal; eauto.
+              econstructor; eauto. constructor.
+          }
+          admit.                (* cases jmp, i.e. tailcall *)
+      + inv SEQ.                (* builtin *)
+        left. eexists; split.
+        * apply plus_one.
+          eapply exec_step_builtin; rewrite <- ? REQ; eauto.
+          eapply eval_builtin_args_eq_rs; eauto.
+        * apply match_states_regular; auto.
+          -- constructor. intros. apply nextinstr_nf_eq.
+             intros. apply set_res_eq.
+             intros; apply undef_regs_eq; auto.
+          -- (* noalloc or ret *)
+            intros sk A; inv A. 2: split; congruence.
+            unfold nextinstr_nf in H6.
+            rewrite Asmgenproof0.nextinstr_pc in H6. simpl in H6. simpl_regs_in H6.
+            setoid_rewrite set_res_other in H6.
+            erewrite Asmgenproof0.undef_regs_other in H6.
+            rewrite H in H6. simpl in H6. inv H6.
+            rewrite_hyps.
+            inv H10; try (now intuition congruence).
+            eapply pallocframe_only_at_beginning in H8; eauto.
+            contradict H8. admit.
+            admit. (* ret is always preceded by freeframe. *)
+            Transparent destroyed_by_builtin.
+            intros r' IN EQ. subst. contradict IN.
+            unfold destroyed_by_builtin. repeat destr; simpl; try intuition congruence.
+            clear. induction clobbers; simpl; intros. inversion 1.
+            destr. simpl. intros [A|A]. destruct m; simpl in A; try congruence. auto.
+            admit.              (* res <> PC *)
+      + admit. (* external *)
+    - inv CL. inv H2.
+      + (* call_s *)
+        inv STEP0; try congruence.
+        rewrite_hyps. simpl in H7. inv H7.
+        destruct (calls_to_defined_functions _ _ _ _ _ H0 H1) as (bf & f' & SA & FFP).
+        assert (bf = b0).
+        {
+          unfold Genv.symbol_address in SA; rewrite FS in SA. inv SA; auto.
+        }
+        subst.
+        inv SEQ.
+        inv STEP; try congruence.
+        * simpl_regs_in H4. rewrite_hyps.
+          exploit pallocframe_at_beginning; eauto. intro FI. setoid_rewrite FI in H6. inv H6.
+          left. simpl in H9. repeat destr_in H9.
+          eexists. split.
+          -- eapply plus_two.
+             eapply exec_step_internal. rewrite <- REQ; eauto. eauto. eauto. simpl.
+             simpl_regs_in Heqo.
+             rewrite Val.offset_ptr_assoc in Heqo.
+             rewrite Ptrofs.add_commut in Heqo.
+             rewrite <- Ptrofs.sub_add_opp in Heqo.
+             rewrite ptrofs_sub_sub in Heqo.
+             rewrite ! REQ in Heqo. rewrite Heqo. eauto.
+             eapply exec_step_internal.
+             simpl_regs. eauto. eauto. eauto.
+             simpl. eauto.
+             reflexivity.
+          -- eapply match_states_regular.
+             ++ constructor.
+                apply nextinstr_eq. simpl_regs.
+                intros. apply set_reg_eq.
+                intros. apply set_reg_eq.
+                intros. rewrite (Pregmap.gso _ _ H2).
+                apply set_reg_eq.
+                intros; apply set_reg_eq. auto.
+                rewrite REQ; auto.
+                auto.
+                auto.
+                rewrite REQ.
+                rewrite Val.offset_ptr_assoc.
+                rewrite <- Ptrofs.neg_add_distr. f_equal.
+                f_equal.
+                generalize (Ptrofs.repr (align (frame_size (fn_frame f)) 8)).
+                generalize (Ptrofs.repr (size_chunk Mptr)). clear.
+                intros.
+                rewrite Ptrofs.sub_add_opp.
+                rewrite (Ptrofs.add_commut i0).
+                rewrite <- Ptrofs.add_assoc.
+                rewrite <- Ptrofs.sub_add_opp. rewrite Ptrofs.sub_idem.
+                rewrite Ptrofs.add_zero_l; auto.
+             ++ intros sk CL. inv CL; try intuition congruence.
+                revert H4. rewrite Asmgenproof0.nextinstr_pc.
+                simpl_regs. rewrite SA. simpl. rewrite Ptrofs.add_zero_l. intro A; inv A.
+                inv H8; try intuition congruence.
+                ** eapply pallocframe_only_at_beginning in H6; eauto.
+                   contradict H6.
+                   rewrite Ptrofs.unsigned_repr by apply instr_size_repr.
+                   apply instr_size_not_zero.
+                ** admit. (*ret not just after builtin *)
+        * rewrite SA in H4. rewrite Pregmap.gss in H4. inv H4. rewrite_hyps.
+          erewrite pallocframe_at_beginning in H6; eauto; inv H6.
+        * rewrite SA in H4. rewrite Pregmap.gss in H4. inv H4. rewrite_hyps.
+          admit.
+      + admit. (* same thing with call_r *)
+    -  
+
+  Qed.
+
+  Lemma real_instr:
+    forall m1 m2 rs1 rs2 f i rs1' m1'
+      (MS: match_states (State rs1 m1) (State rs2 m2))
+      b o
+      (RPC: rs1 PC = Vptr b o)
+      (FFP: Genv.find_funct_ptr ge b = Some (Internal f))
+      (FI: find_instr (Ptrofs.unsigned o) (fn_code f) = Some i)
+      (EI: RawAsm.exec_instr ge f i rs1 m1 = Next rs1' m1')
+,
+      exists rs2' m2',
+        RealAsm.exec_instr ge f i rs2 m2 = Next rs2' m2'
+        /\ match_states (State rs1' m1') (State rs2' m2').
+  Proof.
+    intros m1 m2 rs1 rs2 f i rs1' m1' MS b o RPC FFP FI EI.
+    destruct (instr_same i) eqn:SAME. eapply real_instr_same; eauto.
+    destruct i; simpl in SAME; inv SAME.
+    - destruct (calls_to_defined_functions _ _ _ _ _ FFP FI)
+        as (bf & SA & FFP').
+      destr_in FFP'.
+      destr_in FFP'.
+      + (* call to internal function *)
+        assert (CS: classify_state rs1 = SKcall bf sg).
+        {
+          unfold classify_state. rewrite RPC, FFP, FI.
+          simpl. unfold Genv.symbol_address in SA; repeat destr_in SA.
+        }
+        inv MS; try congruence.
+        destruct RAWSTEP as (rs2' & m2' & RAWSTEP2).
+        inversion RAWSTEP2; try congruence. subst.
+        rewrite <- REQ in H3. rewrite_hyps.
+        do 2 eexists; split. eauto.
+        simpl in EI; inv EI.
+        eapply match_states_alloc.
+        * unfold classify_state.
+          rewrite Pregmap.gss.
+          rewrite SA, Heqo0, FFP'. simpl. eauto.
+        * intros rs0 m1 t STEP.
+          inv STEP; try congruence.
+          Focus 2. rewrite Pregmap.gss in H3. congruence.
+          Focus 2. rewrite Pregmap.gss in H3. congruence.
+          rewrite Pregmap.gss in H3. rewrite SA in H3; inv H3.
+          rewrite Heqo0 in H5; inv H5.
+            rewrite FFP'  in H6; inv H6.
+            simpl in H7. repeat destr_in H7.
+            repeat rewrite Pregmap.gso in Heqo2 by congruence.
+            rewrite Pregmap.gss in Heqo2.
+            rewrite Val.offset_ptr_assoc in Heqo2.
+            rewrite Ptrofs.add_commut in Heqo2.
+            rewrite <- Ptrofs.sub_add_opp in Heqo2.
+            rewrite ptrofs_sub_sub in Heqo2.
+            rewrite ! REQ in Heqo2. rewrite Heqo1 in Heqo2. inv Heqo2.
+            do 2 eexists. split.
+            + econstructor. repeat rewrite Pregmap.gso by congruence. rewrite Pregmap.gss. eauto. eauto.
+              eauto. simpl. eauto.
+            + constructor.
+              apply nextinstr_eq.
+              repeat rewrite Pregmap.gso by congruence.
+              repeat rewrite Pregmap.gss.
+              intros. apply set_reg_eq.
+              intros. apply set_reg_eq.
+              intros. rewrite (Pregmap.gso _ _ H).
+              apply set_reg_eq.
+              intros; apply set_reg_eq. auto.
+              rewrite REQ; auto.
+              auto.
+              auto.
+              rewrite REQ.
+              rewrite Val.offset_ptr_assoc.
+              rewrite <- Ptrofs.neg_add_distr. f_equal.
+              f_equal.
+              generalize (Ptrofs.repr (align (frame_size (fn_frame f0)) 8)).
+              generalize (Ptrofs.repr (size_chunk Mptr)). clear.
+              intros.
+              rewrite Ptrofs.sub_add_opp.
+              rewrite (Ptrofs.add_commut i0).
+              rewrite <- Ptrofs.add_assoc.
+              rewrite <- Ptrofs.sub_add_opp. rewrite Ptrofs.sub_idem.
+              rewrite Ptrofs.add_zero_l; auto.
+              unfold classify_state.
+              rewrite Asmgenproof0.nextinstr_pc.
+              repeat rewrite Pregmap.gso by congruence.
+              rewrite Pregmap.gss. rewrite SA. simpl.
+              rewrite Heqo0.
+              destr.
+              destruct i; auto.
+              eapply pallocframe_only_at_beginning in Heqo2; eauto.
+              rewrite Ptrofs.add_zero_l in Heqo2.
+              simpl in Heqo2.
+              rewrite Ptrofs.unsigned_repr in Heqo2.
+              2: apply instr_size_repr.
+
+              Lemma instr_size_not_zero:
+                forall i,
+                  instr_size i <> 0.
+              Proof.
+                intros; apply not_eq_sym; apply Z.lt_neq, instr_size_positive.
+              Qed.
+
+              apply instr_size_not_zero in Heqo2. easy.
+        }
+        
+
+      + intros.
+        setoid_rewrite Pregmap.gsspec. repeat destr; subst.
+        repeat setoid_rewrite Pregmap.gsspec. repeat destr; subst.
+        repeat setoid_rewrite Pregmap.gsspec. repeat destr; subst.
+        repeat setoid_rewrite Pregmap.gsspec. admit.
+        repeat setoid_rewrite Pregmap.gsspec. repeat destr; subst.
+        setoid_rewrite Pregmap.gso . 2: congruence.
+        rewrite Pregmap.gss. rewrite REQ. auto.
+
+
+        simpl.
+
+      admit.
+    - admit.
+    - admit.
+    - assert (classify_state rs1 = SKalloc frame ofs_ra).
+      unfold classify_state. rewrite RPC, FFP, FI; reflexivity.
+      inv MS; try congruence.
+      edestruct RAWSTEP as (rs4 & m4 & STEP & MS').
+      econstructor; eauto.
+      inv STEP; try congruence.
+      rewrite <- REQ, RPC in H4 ; inv H4.
+      rewrite FFP in H5; inv H5.
+      rewrite FI in H6; inv H6.
+      rewrite H7. do 2 eexists; split; eauto.
+    -
+  Qed.
+    
+
+  
+  Lemma instr_correct:
+    forall 
+
+  
+  Lemma ZEQ: forall a b,
+      proj_sumbool (zeq a b) = true -> a = b.
+  Proof.
+    intros; destruct zeq; auto. discriminate.
+  Qed.
+
+  Lemma ZLE: forall a b c d,
+      zle a b || zle c d = true ->
+      a <= b \/ c <= d.
+  Proof.
+    intros; destruct (zle a b), (zle c d); try congruence; try omega.
+    simpl in H; congruence.
+  Qed.
+
+  Lemma perm_stack_eq':
+    forall l m b fi j
+      (SAP: stack_agree_perms (Mem.perm m) l)
+      (PS: inject_perm_stack j (Mem.perm m) l)
+      (INBLOCKS: in_stack' l (b, fi))
+      o k p,
+      Mem.perm m b o k p <-> 0 <= o < frame_size fi.
+  Proof.
+    induction 2; simpl; intros; eauto.
+    - easy.
+    - destruct INBLOCKS as [EQ | INSTK]. easy. 
+      eapply IHPS; eauto. red; intros; eapply SAP; eauto. right; eauto.
+    - destruct INBLOCKS as [EQ | INSTK].
+      + red in EQ. simpl in EQ.
+        red in EQ. rewrite BLOCKS in EQ. destruct EQ as [A|[]]; inv A.
+        split. 2: apply PERM. eapply SAP. left. reflexivity. reflexivity.
+        rewrite BLOCKS. left; reflexivity.
+      + eapply IHPS; eauto. red; intros; eapply SAP; eauto. right; eauto.
+  Qed.
+
+  Lemma perm_stack_eq:
+    forall m b fi j
+      (PS: inject_perm_stack j (Mem.perm m) (Mem.stack m))
+      (INBLOCKS: in_stack' (Mem.stack m) (b, fi))
+      o k p,
+      Mem.perm m b o k p <-> 0 <= o < frame_size fi.
+  Proof.
+    intros; eapply perm_stack_eq'; eauto.
+    apply Mem.agree_perms_mem.
+  Qed.
+  
+  Lemma size_stack_app:
+    forall l1 l2,
+      StackADT.size_stack (l1 ++ l2) = StackADT.size_stack l1 + StackADT.size_stack l2.
+  Proof.
+    induction l1; simpl; intros; eauto.
+    rewrite IHl1. omega.
+  Qed.
+
+  Lemma val_inject_set:
+    forall j rs1 rs2 r0 r1
+      (RINJ: r0 <> r1 -> Val.inject j (rs1 r0) (rs2 r0))
+      v v' (VINJ: Val.inject j v v'),
+      Val.inject j ((rs1 # r1 <- v) r0) ((rs2 # r1 <- v') r0).
+  Proof.
+    intros.
+    destruct (PregEq.eq r1 r0); subst; auto.
+    rewrite ! Pregmap.gss; auto.
+    rewrite ! Pregmap.gso by auto. auto.
+  Qed.
+
+  Lemma val_inject_undef_regs:
+    forall l j rs1 rs2
+      (RINJ: forall r, Val.inject j (rs1 r) (rs2 r))
+      r,
+      Val.inject j (undef_regs l rs1 r) (undef_regs l rs2 r).
+  Proof.
+    induction l; simpl; intros; eauto.
+    apply IHl.
+    intros; apply val_inject_set; auto.
+  Qed.
+
+  Lemma val_inject_nextinstr:
+    forall j rs1 rs2 r sz
+      (RINJ: forall r0, r0 = r \/ r0 = PC -> Val.inject j (rs1 r0) (rs2 r0)),
+      Val.inject j (nextinstr rs1 sz r) (nextinstr rs2 sz r).
+  Proof.
+    unfold nextinstr.
+    intros.
+    apply val_inject_set; auto. 
+    apply Val.offset_ptr_inject; auto.
+  Qed.
+
+  Lemma find_var_info_none_ge:
+    forall b,
+      (Genv.genv_next ge <= b)%positive ->
+      Genv.find_var_info ge b = None.
+  Proof.
+    unfold Genv.find_var_info. intros.
+    destr.
+    apply Genv.genv_defs_range in Heqo. xomega.
+  Qed.
+
+  Lemma load_record_stack_blocks:
+    forall m fi m',
+      Mem.record_stack_blocks m fi = Some m' ->
+      forall chunk b ofs,
+        Mem.load chunk m' b ofs = Mem.load chunk m b ofs.
+  Proof.
+    intros.
+    destruct (plt b (Mem.nextblock m)).
+    eapply Mem.load_unchanged_on_1.
+    eapply Mem.strong_unchanged_on_weak.
+    eapply Mem.record_stack_block_unchanged_on; eauto.
+    apply p.
+    instantiate (1 := fun _ _ => True); simpl; auto.
+    destruct (Mem.load chunk m b ofs) eqn:LOAD.
+    apply Mem.load_valid_access in LOAD. destruct LOAD.
+    exfalso; apply n.
+    eapply Mem.perm_valid_block. apply H0.
+    instantiate (1:= ofs). generalize (size_chunk_pos chunk); omega.
+    clear LOAD.
+    destruct (Mem.load chunk m' b ofs) eqn:LOAD; auto.
+    apply Mem.load_valid_access in LOAD. destruct LOAD.
+    exfalso; apply n.
+    eapply Mem.perm_valid_block.
+    specialize (H0 ofs). trim H0. generalize (size_chunk_pos chunk); omega.
+    rewrite_perms_bw H0.
+    apply H0.
+  Qed.
+  
+  Lemma size_frames_nil: size_frames (None,nil) = 0.
+  Proof.
+    reflexivity.
+  Qed.
+
+  Lemma size_frames_one:
+    forall f,
+      size_frames (Some f , nil) = align (frame_adt_size f) 8.
+  Proof.
+    intros. rewrite size_frames_cons. simpl. unfold size_frame.
+    apply Z.max_l. etransitivity.
+    2: apply align_le.
+    apply frame_adt_size_pos. omega.
+  Qed.
+
+  Opaque Mem.stack_limit.
+
+
+
+  Lemma in_stack_inj_below:
+    forall j P l
+      (IS: inject_perm_stack j P l)
+      b fi
+      (INFRAMES: in_stack' l (b,fi)),
+    exists l1 l2,
+      l = l1 ++ l2 /\
+      j b = Some (bstack, Mem.stack_limit - size_active_stack l2).
+  Proof.
+    induction 1; simpl; intros; eauto. easy.
+    - destruct INFRAMES as [[]|INFRAMES].
+      edestruct IHIS as (l1 & l2 & EQ & JB); eauto.
+      exists ((None,r)::l1),l2; split; auto. simpl. subst. reflexivity.
+    - destruct INFRAMES as [IFR|INSTACK].
+      + red in IFR. simpl in IFR.
+        red in IFR. rewrite BLOCKS in IFR.
+        destruct IFR as [EQ|[]]. inv EQ.
+        rewrite JB.
+        exists nil, ((Some fr, r)::l). simpl. split; auto.
+        unfold size_frame. rewrite SIZE. f_equal. f_equal. omega.
+      + edestruct IHIS as (l1 & l2 & EQ & JB'); eauto.
+        exists ((Some fr,r)::l1),l2; split; auto. simpl. subst. reflexivity.
+  Qed.
+
+  Lemma size_active_smaller:
+    forall s,
+      size_active_stack s <= size_stack s.
+  Proof.
+    induction s; simpl; intros; eauto. omega.
+    apply Z.add_le_mono; auto.
+    destruct a; simpl. rewrite size_frames_cons.
+    apply Z.le_max_l.
+  Qed.
+
+  Lemma size_active_stack_below:
+    forall m,
+      size_active_stack (Mem.stack m) < Mem.stack_limit.
+  Proof.
+    intros. eapply Z.le_lt_trans.
+    2: apply Mem.size_stack_below.
+    apply size_active_smaller.
+  Qed.
+
+  Lemma size_active_stack_pos:
+    forall s,
+      0 <= size_active_stack s.
+  Proof.
+    induction s; simpl; intros; eauto. omega.
+    generalize (opt_size_frame_pos (fst a)); omega.
+  Qed.
+  
+  Lemma size_frame_rew:
+    forall b fi fr,
+      size_frame (make_singleton_frame_adt' b fi (frame_size fr)) = align (frame_size fr) 8.
+  Proof.
+    unfold size_frame; simpl. intros.
+    rewrite Z.max_r; auto.
+    apply frame_size_pos.
+  Qed.
+
+  Lemma align_frame_size_pos:
+    forall fr,
+      0 <= align (frame_size fr) 8.
+  Proof.
+    intros.
+    etransitivity.
+    2: apply align_le; try omega.
+    apply frame_size_pos.
+  Qed.
+  
+ Lemma alloc_inject:
+    forall j ostack m1 (rs1 rs1': regset) fi b m1' m5 ofs_ra m2 m4 sz,
+      match_states j (Ptrofs.unsigned ostack) (State rs1 m1) (State rs1' m1') ->
+      top_tframe_tc (Mem.stack m1) ->
+      Mem.alloc m1 0 (frame_size fi) = (m2, b) ->
+      Mem.store Mptr m2 b ofs_ra rs1#RA = Some m4 ->
+      Mem.record_stack_blocks m4 (make_singleton_frame_adt' b  fi (frame_size fi)) = Some m5 ->
+      0 <= ofs_ra <= Ptrofs.max_unsigned ->
+      0 < frame_size fi ->
+      let sp := Val.offset_ptr (rs1' RSP) (Ptrofs.neg (Ptrofs.repr (align (frame_size fi) 8))) in
+      let newostack := Ptrofs.unsigned ostack - align (frame_size fi) 8 in
+      let rs2 := nextinstr ( rs1 #RAX <- (rs1#RSP)  #RSP <- (Vptr b Ptrofs.zero)) sz in
+      let rs2' := nextinstr (rs1' #RAX <- (rs1'#RSP) #RSP <- sp) sz in
+      exists j',
+        (forall bb, j' bb = if peq bb b then Some (bstack, newostack) else j bb)
+        /\ inject_incr j j'
+        /\
+        exists m4',
+          Mem.storev Mptr m1' (Val.offset_ptr sp (Ptrofs.repr ofs_ra)) rs1'#RA = Some m4'
+          /\ match_states j' newostack (State rs2 m5) (State rs2' m4').
+  Proof.
+    intros j ostack m1 rs1 rs1' fi b m1' m5 ofs_ra m2 m4 sz
+           MS TIN ALLOC STORE RSB REPRretaddr sizepos
+           sp newostack rs2 rs2'.
+    inv MS.
+    assert (RNGframe: 0 <= align (frame_size fi) 8 <= Ptrofs.max_unsigned).
+    {
+      split. apply align_frame_size_pos.
+      etransitivity. 2: eapply Z.lt_le_incl, Z.lt_le_trans.
+      2: apply (size_active_stack_below m5).
+      repeat rewrite_stack_blocks. simpl.
+      rewrite size_frame_rew. generalize (size_active_stack_pos r). intros; omega.
+      apply Mem.stack_limit_range.
+    }
+    assert (SP: sp = Vptr bstack (Ptrofs.repr newostack)).
+    {
+      unfold sp. rewrite RSPEQ. simpl. f_equal.
+      rewrite <- Ptrofs.sub_add_opp. unfold newostack.
+      unfold Ptrofs.sub. rewrite H1. rewrite Ptrofs.unsigned_repr; auto.
+    }
+    assert (REPRcur: align (frame_size fi) 8 <= Ptrofs.unsigned ostack0 <= Ptrofs.max_unsigned).
+    {
+      split. 2: apply Ptrofs.unsigned_range_2.
+      red in AGSP. specialize (AGSP _ RSPEQ). rewrite AGSP.
+      apply Z.le_add_le_sub_r.
+      eapply Z.lt_le_incl, Z.le_lt_trans. 2: apply (size_active_stack_below m5).
+      repeat rewrite_stack_blocks. intro. 
+      simpl. rewrite EQ1. simpl. rewrite size_frame_rew. omega.
+    }
+    assert (REPR: 0 <= newostack <= Ptrofs.max_unsigned).
+    {
+      unfold newostack. omega.
+    }
+    generalize (Mem.alloc_left_mapped_inject _ _ _ _ _ _ _ _ _ newostack MINJ ALLOC VB).
+    intro A.
+    trim A. now omega.
+    trim A. intros; right; eapply PBS; now eauto.
+    trim A.
+    {
+      intros; eapply Mem.perm_implies. eapply PBSL; eauto.
+      split. omega.
+      unfold newostack.
+      eapply Z.lt_le_trans with (Ptrofs.unsigned ostack).
+      cut (frame_size fi <= align (frame_size fi) 8). omega.
+      apply align_le. omega.
+      erewrite <- H1, (AGSP _ RSPEQ); eauto.
+      generalize (size_active_stack_pos (Mem.stack m1)); intros. omega.
+      simpl in H0. auto.
+    }
+    trim A.
+    {
+      red.
+      intros.
+      unfold newostack.
+      eapply Zdivides_trans with 8.
+      destruct chunk; try (exists 8; reflexivity);
+        try (exists 4; reflexivity);
+        try (exists 2; reflexivity);
+        try (exists 1; reflexivity).
+      apply Z.divide_sub_r.
+      rewrite <- H1. apply SPAL; auto.
+      apply align_divides. omega.
+    }
+    trim A.
+    {
+      intros b0 delta' ofs k p JB PERM RNG.
+      generalize (NIB _ _ _ _ _ JB PERM).
+      generalize (align_le (frame_size fi) 8).
+      unfold newostack in RNG. simpl in RNG. omega.
+    }
+    trim A.
+    {
+      revert NS. unfold no_stack.
+      intros (fr & fi0 & rr & EQS & BLOCKS & ZERO & PUBLIC & SIZE). rewrite EQS.
+      simpl. intros fi1 [INFR|INS]; subst.
+      - red in INFR.  simpl in INFR. red in INFR; revert INFR.
+        rewrite <- BLOCKS.
+        intros [EQ|[]]. inv EQ.
+        intros; apply PUBLIC.
+      - exploit Mem.stack_norepet. rewrite EQS.
+        intro ND; inv ND.
+        exfalso; eapply H3. 2: eapply in_stack'_in_stack; apply INS.
+        red; simpl. unfold get_frame_blocks. rewrite <- BLOCKS. left; reflexivity.
+    }
+    destruct A as (f' & MINJ' & INCR & EQ1 & EQ2).
+    exists f'.
+    split.
+    {
+      intros.
+      destruct peq; subst; eauto.
+    }
+    split; auto.
+    (* store return address *)
+    exploit Mem.store_mapped_inject. apply MINJ'. simpl in *; eauto. eauto. 
+    eapply val_inject_incr; eauto. intros (m4' & STORE' & MINJ3).
+    assert (Ptrofs.unsigned (Ptrofs.add (Ptrofs.repr newostack) (Ptrofs.repr ofs_ra)) =
+            ofs_ra + newostack) as EQ'.
+    2: simpl. 
+    rewrite Ptrofs.add_commut.
+    erewrite Mem.address_inject; eauto.
+    rewrite Ptrofs.unsigned_repr; omega.
+    exploit Mem.store_valid_access_3. exact STORE.
+    intro VA; eapply Mem.store_valid_access_1 in VA; eauto. destruct VA.
+    eapply H. 
+    rewrite Ptrofs.unsigned_repr; generalize (size_chunk_pos Mptr); omega.
+    rewrite SP. simpl. unfold Ptrofs.add.
+    rewrite (Ptrofs.unsigned_repr _ REPR).
+    rewrite (Ptrofs.unsigned_repr _ REPRretaddr) in *.
+    rewrite Ptrofs.unsigned_repr. rewrite Z.add_comm. rewrite STORE'.
+    eexists; split; eauto.
+    (* record the stack block *)
+    destruct NS as (frstack & fstack & rr & EQstk & BLOCKS & ZERO & PUB & SZ).
+    exploit Mem.record_stack_block_inject_left_zero. apply MINJ3. 3: eauto.
+    repeat rewrite_stack_blocks. rewrite EQstk. constructor; reflexivity.
+    {
+      red. simpl.
+      intros ? EQ HPF. inv EQ.
+      exists frstack; split; auto.
+      red. simpl.
+      constructor; auto. simpl. rewrite EQ1.
+      intros b2 delta A; inv A.
+      rewrite <- BLOCKS. simpl.
+      eexists; split. eauto.
+      constructor.
+      intros; eapply stack_perm_le_public. intros; apply PUB.
+      intros; rewrite SZ.
+      unfold newostack.
+      rewrite <- H1.
+      red in AGSP. apply AGSP in RSPEQ.  rewrite RSPEQ.
+      cut (frame_size fi <= align (frame_size fi) 8).
+      generalize (size_active_stack_pos (Mem.stack m1)). omega.
+      apply align_le; omega.
+    }
+    intro MINJ4.
+    (* proving the final match_states *)
+    rewrite <- (Ptrofs.unsigned_repr newostack) by omega.
+    destruct lprog.
+    {
+      revert init_sp_ptr. unfold init_sp. simpl in STK. subst.
+      clear STK. inv TIN. simpl. unfold current_frame_sp; rewrite H0. inversion 1.
+    }
+    simpl in STK.
+    assert (
+        Mem.stack m5 = (Some (make_singleton_frame_adt' b fi (frame_size fi)), opt_cons (fst t) (snd t)) :: lprog ++ init_stk
+        /\ Mem.stack m1 = (None, (snd t)) :: lprog ++ init_stk
+      ).
+    {
+      repeat rewrite_stack_blocks.
+      rewrite STK. inversion 1; subst. simpl. auto.
+    }
+    destruct H as (STK5 & STK1).
+    econstructor. eauto.
+    - rewrite STK5. rewrite app_comm_cons. reflexivity.
+    - simpl. reflexivity.
+    - unfold rs2. rewrite nextinstr_rsp, Pregmap.gss. eauto.
+    - intros r.
+      unfold rs2, rs2'.
+      apply val_inject_nextinstr. intros.
+      apply val_inject_set; eauto. intro. apply val_inject_set. intros; eauto.
+      eapply val_inject_incr; eauto.
+      subst sp. simpl. rewrite RSPEQ. econstructor; eauto. rewrite Ptrofs.add_zero_l; auto.
+      unfold newostack. rewrite <- Ptrofs.sub_add_opp. unfold Ptrofs.sub. rewrite <- H1. rewrite Ptrofs.unsigned_repr; auto.
+    - red. rewnb. eauto.
+    - red. unfold rs2'. rewrite nextinstr_rsp. rewrite Pregmap.gss. rewrite SP. inversion 1. subst.
+      repeat rewrite_stack_blocks.
+      rewrite Ptrofs.unsigned_repr by auto.
+      unfold newostack in *.
+      rewrite <- H1. rewrite (AGSP _ RSPEQ).
+      intro EQ0; rewrite EQ0. simpl. rewrite size_frame_rew. omega.
+    - red. intros ostack1 A. unfold rs2' in A. rewrite nextinstr_rsp in A. rewrite Pregmap.gss in A.
+      rewrite SP in A. inversion A. subst.
+      rewrite Ptrofs.unsigned_repr by omega.
+      unfold newostack.
+      apply Z.divide_sub_r. rewrite <- H1. apply SPAL. auto.
+      apply align_divides. omega.
+    - red. intros ofs k p PERM.
+      repeat rewrite_perms_bw PERM. eauto.
+    - red; intros.
+      repeat rewrite_perms_fw. eauto.
+    - red. repeat rewrite_stack_blocks. exists frstack, fstack, rr; rewrite EQstk, <- BLOCKS, <- ZERO. eauto.
+    - unfold rs2'. rewrite nextinstr_rsp, Pregmap.gss. auto.
+    - rewrite Ptrofs.unsigned_repr by omega.
+      red. intros b0 delta o k p JB PERM.
+      repeat rewrite_perms_bw PERM.
+      destruct peq.
+      * subst. rewrite EQ1 in JB. clear EQstk. inv JB. split. omega.
+        rewrite STK5. rewrite in_stack_cons. rewrite in_frames_cons.
+        left. eexists; split; eauto. unfold in_frame; simpl; auto.
+      * split. unfold newostack.
+        transitivity (Ptrofs.unsigned ostack).
+        -- generalize (align_le ((frame_size fi)) 8). omega.
+        -- rewrite <- H1.
+          rewrite EQ2 in JB; auto. 
+          exploit NIB; eauto. tauto.
+        -- rewrite STK5.
+           rewrite in_stack_cons.
+           right.
+           edestruct NIB; eauto. rewrite <- EQ2; eauto.
+           rewrite STK1 in H0. rewrite in_stack_cons in H0. destruct H0; auto. easy.
+    - rewrite STK5.
+      rewrite STK1 in IS. inv IS. 
+      econstructor; try reflexivity; eauto.
+      eapply inject_stack_incr; eauto.
+      eapply inject_stack_more_perm with (P:=Mem.perm m1).
+      intros; repeat rewrite_perms.
+      exploit Mem.perm_valid_block; eauto. intro VB'.
+      generalize (Mem.fresh_block_alloc _ _ _ _ _ ALLOC). destr. auto.
+      rewrite EQ1. f_equal. f_equal.
+      unfold newostack.
+      rewrite <- H1.
+      rewrite AGSP. rewrite STK1. simpl. omega. auto. 
+      simpl. rewrite Z.max_r; auto. omega.
+      intros. repeat rewrite_perms. destr.
+    - intros b0 fi0 delta INSTK FB0 b' o delta' k p FB1 P1.
+      revert INSTK. rewrite STK5. intro INSTK.
+      simpl in INSTK.
+      repeat rewrite_perms_bw P1.
+      destruct INSTK as [IFR|INSTK].
+      + red in IFR. simpl in IFR. red in IFR. simpl in IFR. destruct IFR as [EQ|[]]. inv EQ.
+        rewrite FB0 in EQ1; inv EQ1.
+        destr_in P1.
+        * subst. rewrite FB0 in FB1; inv FB1. omega.
+        * rewrite EQ2 in FB1 by auto.
+          eapply NIB in P1; eauto.
+          destruct P1 as (LE & IN).
+          unfold newostack.
+          rewrite <- H1.
+          omega.
+      + assert (b0 <> b). intro; subst.
+        exploit Mem.stack_norepet. rewrite STK5. intro ND; inv ND.
+        eapply in_stack'_in_stack in INSTK; eauto. eapply H3 in INSTK; eauto.
+        left. reflexivity.
+        rewrite EQ2 in FB0 by auto.
+        intro RNG.
+        assert (0 < frame_size fi0).
+        destruct (zlt 0 (frame_size fi0)); auto.
+        assert (frame_size fi0 = 0). generalize (frame_size_pos fi0); omega. rewrite H0 in RNG.
+        change (align 0 8) with 0 in RNG. omega.
+        destr_in P1. 
+        * subst. rewrite EQ1 in FB1; inv FB1.
+          cut (newostack + (frame_size fi)  <= delta). omega.
+          unfold newostack. rewrite <- H1.
+          rewrite AGSP; auto.
+          rewrite STK1 in IS. inv IS.
+          eapply in_stack_inj_below in INSTK; eauto.
+          destruct INSTK as (l1 & l2 & EQADT & JB0). rewrite FB0 in JB0. inv JB0.
+          rewrite STK1. simpl. rewrite EQADT.
+
+          Lemma size_active_stack_app:
+            forall l1 l2,
+              size_active_stack (l1 ++ l2) = size_active_stack l1 + size_active_stack l2.
+          Proof.
+            induction l1; simpl; intros; eauto.
+            rewrite IHl1. omega.
+          Qed.
+          rewrite size_active_stack_app.
+          generalize (size_active_stack_pos l1).
+          cut (frame_size fi <= align (frame_size fi) 8). omega.
+          apply align_le; omega.
+        * eapply IP. rewrite STK1. right. eauto. eauto.
+          rewrite <- EQ2. apply FB1. auto. eauto. omega.
+    - eauto.
+    - eauto.
+    - destruct GLOBSYMB_INJ; split.
+      + intros. eapply INCR. eauto.
+      + intros. destruct (peq b1 b).
+        subst; rewrite EQ1 in H2. clear EQstk. inv H2.
+        simpl.
+        unfold Genv.block_is_volatile.
+        unfold Genv.find_var_info.
+        replace (Genv.find_def ge bstack) with (None (A:=globdef Asm.fundef unit)).
+        replace (Genv.find_def ge b) with (None (A:=globdef Asm.fundef unit)).
+        auto.
+        unfold Genv.find_def.
+        destruct (Maps.PTree.get b (Genv.genv_defs ge)) eqn:EQdef; auto.
+        apply Genv.genv_defs_range in EQdef.
+        exploit Mem.fresh_block_alloc. eauto. red. xomega. easy.
+        unfold Genv.find_def.
+        destruct (Maps.PTree.get bstack (Genv.genv_defs ge)) eqn:EQdef; auto.
+        apply Genv.genv_defs_range in EQdef.
+        unfold bstack in EQdef. xomega.
+        rewrite EQ2 in H2.
+        eauto.
+        auto.
+    - erewrite Mem.record_stack_block_nextblock. 2: eauto.
+      erewrite Mem.nextblock_store. 2 : eauto.
+      erewrite Mem.nextblock_alloc. 2: eauto. xomega.
+    - erewrite Mem.nextblock_store. 2 : eauto. xomega.
+    - rewrite STK5. simpl. right. rewrite STK1 in SPinstack. destruct SPinstack; auto. easy.
+    - rewrite Z.add_comm, <- EQ'. apply Ptrofs.unsigned_range_2.
+  Qed.
+
+  Lemma max_l_divide l: (8 | max_l (map size_frame l)).
+  Proof.
+    induction l; simpl. exists 0; omega.
+    rewrite Zmax_spec.
+    destr.
+    apply align_divides. omega.
+  Qed.
+  
+  Lemma opt_size_frame_divides f:
+    (8 | opt_size_frame f).
+  Proof.
+    destruct f.
+    apply align_divides. omega.
+    exists 0; simpl; omega.
+  Qed.
+
+  Lemma size_frames_divides f:
+    (8 | size_frames f).
+  Proof.
+    unfold size_frames.
+    destruct f; simpl. 
+    rewrite Zmax_spec.
+    destr.
+    apply opt_size_frame_divides.
+    apply max_l_divide.
+  Qed.
+
+  Lemma size_stack_divides l:
+    (8 | size_stack l).
+  Proof.
+    induction l; simpl; intros; eauto.
+    exists 0; omega.
+    apply Z.divide_add_r. auto. apply size_frames_divides; auto.
+  Qed.
+
+  Lemma size_active_stack_divides l:
+    (8 | size_active_stack l).
+  Proof.
+    induction l; simpl; intros; eauto.
+    exists 0; omega.
+    apply Z.divide_add_r. auto. apply opt_size_frame_divides.
+  Qed.
+  
+  Lemma inject_stack_init_sp:
+    forall j P l,
+      inject_perm_stack j P l ->
+      forall b,
+        in_stack l b ->
+        exists o,
+          j b = Some (bstack, o).
+  Proof.
+    induction 1; simpl; intros bb INS. easy.
+    rewrite in_stack_cons in INS. destruct INS as [INF|INS]. easy. eauto.
+    rewrite in_stack_cons in INS. destruct INS as [INF|INS].
+    rewrite in_frames_cons in INF. destruct INF as (f1 & EQ & IFR); inv EQ.
+    edestruct in_frame_info as (ffi & IFRR). eauto.
+    rewrite BLOCKS in IFRR. destruct IFRR as [IFRR|[]]. inv IFRR. eauto.
+    eauto.
+  Qed.
+
+  Lemma init_sp_inj:
+    forall j P l,
+      inject_perm_stack j P l ->
+      in_stack l binit_sp ->
+      exists o,
+        Val.inject j init_sp (Vptr bstack o).
+  Proof.
+    intros. edestruct inject_stack_init_sp; eauto.
+    rewrite init_sp_ptr. exists (Ptrofs.repr x).
+    econstructor; eauto. rewrite Ptrofs.add_zero_l. auto.
+  Qed.
+
+  Ltac use_ains :=
+    repeat match goal with
+           | AINS: asm_instr_no_stack ?i,
+                   UNC: stack_invar ?i = true,
+                        EI: Asm.exec_instr ?init_stk _ _ ?i _ ?m1 = Next _ ?m2 |-
+             context [Mem.stack ?m2] =>
+             let AINS_stack := fresh "AINS_stack" in
+             edestruct (AINS UNC _ _ _ _ _ _ _ _ _ EI) as (AINS_stack & _); rewrite ! AINS_stack;
+             clear AINS_stack
+           | AINS: asm_instr_no_stack ?i,
+                   UNC: stack_invar ?i = true,
+                        EI: Asm.exec_instr ?init_stk _ _ ?i _ ?m1 = Next _ ?m2,
+                            H: context [Mem.stack ?m2] |- _ =>
+             let AINS_stack := fresh "AINS_stack" in
+             edestruct (AINS UNC _ _ _ _ _ _ _ _ _ EI) as (AINS_stack & _); rewrite ! AINS_stack in H;
+             clear AINS_stack
+
+           | AINS: asm_instr_no_stack ?i,
+                   UNC: stack_invar ?i = true,
+                        EI: Asm.exec_instr ?init_stk _ _ ?i _ ?m1 = Next _ ?m2 |-
+             context [Mem.perm ?m2 _ _ _ _] =>
+             let AINS_perm := fresh "AINS_perm" in
+             edestruct (AINS UNC _ _ _ _ _ _ _ _ _ EI) as (_ & AINS_perm); rewrite ! AINS_perm;
+             clear AINS_perm
+           | AINS: asm_instr_no_stack ?i,
+                   UNC: stack_invar ?i = true,
+                        EI: Asm.exec_instr ?init_stk _ _ ?i _ ?m1 = Next _ ?m2,
+                            H : context [Mem.perm ?m2 _ _ _ _] |- _ =>
+             let AINS_perm := fresh "AINS_perm" in
+             edestruct (AINS UNC _ _ _ _ _ _ _ _ _ EI) as (_ & AINS_perm); rewrite ! AINS_perm in H;
+             clear AINS_perm
+           | AINR: asm_instr_no_rsp ?i,
+                   UNC: stack_invar ?i = true,
+                        EI: Asm.exec_instr ?init_stk _ _ ?i ?rs1 _ = Next ?rs2 _ |-
+             context [?rs2 (IR RSP)] =>
+             rewrite (AINR UNC _ _ _ _ _ _ _ _ _ EI)
+           | AINR: asm_instr_no_rsp ?i,
+                   UNC: stack_invar ?i = true,
+                        EI: Asm.exec_instr ?init_stk _ _ ?i ?rs1 _ = Next ?rs2 _,
+                            H: context [?rs2 (IR RSP)] |- _ =>
+             rewrite (AINR UNC _ _ _ _ _ _ _ _ _ EI) in H
+                                                          
+           end.
+
+  Lemma is_unchanged_stack_invar:
+    forall i,
+      is_unchanged i = true ->
+      stack_invar i = true.
+  Proof.
+    intros. destruct i. destruct i eqn:?; simpl in *; try congruence.
+  Qed.
+
+  (* Lemma clear_stage_inject_left: *)
+  (*   forall j n g m1 m2 m1', *)
+  (*     Mem.inject j (S n :: g) m1 m2 -> *)
+  (*     le 1 n -> *)
+  (*     Mem.clear_stage m1 = Some m1' -> *)
+  (*     (forall b : block, is_stack_top (Mem.stack m1) b -> forall (o : Z) (k : perm_kind) (p : permission), ~ Mem.perm m1 b o k p) -> *)
+  (*     Mem.inject j (S n :: g) m1' m2. *)
+  (* Proof. *)
+  (*   intros j n g m1 m2 m1' INJ LE CS TOP. *)
+  (*   unfold Mem.clear_stage in CS; repeat destr_in CS. *)
+  (*   apply Mem.inject_push_new_stage_left. *)
+  (*   eapply Mem.unrecord_stack_block_inject_left; eauto. *)
+  (* Qed. *)
+
+  Lemma zle_zlt:
+    forall lo hi o,
+      zle lo o && zlt o hi = true <-> lo <= o < hi.
+  Proof.
+    intros.
+    destruct (zle lo o), (zlt o hi); intuition; try congruence; try omega.
+  Qed.
+
+  Lemma max_align:
+    forall x, 0 <= x ->
+         Z.max 0 (align x 8) = align (Z.max 0 x) 8.
+  Proof.
+    intros.
+    rewrite ! Z.max_r; auto.
+    etransitivity. 2: apply align_le. auto. omega.
+  Qed.
+
+  Lemma mod_divides:
+    forall a b c,
+      c <> 0 ->
+      (a | c) ->
+      (a | b) ->
+      (a | b mod c).
+  Proof.
+    intros.
+    rewrite Zmod_eq_full.
+    apply Z.divide_sub_r. auto.
+    apply Z.divide_mul_r. auto. auto.
+  Qed.
+  
+  Lemma exec_instr_inject':
+    forall j ostack m1 m2 rs1 rs2 f i rs1' m1'
+      (MS: match_states j ostack (State rs1 m1) (State rs2 m2))
+      (AINR: asm_instr_no_rsp i)
+      (AINS: asm_instr_no_stack i)
+      (EI: Asm.exec_instr init_stk ge f i rs1 m1 = Next rs1' m1'),
+      exists j' ostack' rs2' m2',
+        exec_instr ge f i rs2 m2 = Next rs2' m2'
+        /\ match_states j' ostack' (State rs1' m1') (State rs2' m2')
+        /\ inject_incr j j'.
+  Proof.
+    intros. 
+    destruct (is_unchanged i) eqn:ISUNCH.
+    - inversion MS.
+      edestruct exec_instr_inject as (rs2' & m2' & EXEC' & MINJ' & RINJ'); eauto.
+      exists j, ostack, rs2', m2'; split; [|split]; eauto.
+      destruct i as (i & szinfo); destruct i; simpl in *; eauto; try congruence.
+      generalize (is_unchanged_stack_invar _ ISUNCH) as SINVAR. intro.
+      subst. eapply match_states_intro; eauto; try now ((intros; use_ains; eauto) || (red; intros; use_ains; eauto)).
+      + eapply asmgen_nextblock_forward in EXEC'.
+        red in VB |- *. xomega.
+      + use_ains. 
+        eapply perm_stack_inv. eauto.
+        intros; use_ains. tauto.
+      + etransitivity. apply GlobLe.
+        eapply asmgen_nextblock_forward; eauto.
+      + etransitivity. apply GlobLeT.
+        eapply asmgen_nextblock_forward; eauto.
+        
+    - destruct i as (i & szinfo).
+      destruct i; simpl in *; try congruence.
+      + (* call_s *)
+        inv EI. inv MS. do 4 eexists. split. eauto. split. econstructor; eauto.
+        * instantiate (1:= _::_). simpl. eapply Mem.inject_push_new_stage_left; eauto.
+        * rewrite_stack_blocks. rewrite STK. simpl. reflexivity.
+        * intros; apply val_inject_set; auto.
+          intros; apply val_inject_set; auto.
+          apply Val.offset_ptr_inject; auto.
+          unfold Genv.symbol_address. destr; auto.
+          destruct GLOBSYMB_INJ. apply H in Heqo.
+          econstructor; eauto.
+        * red. rewrite_stack_blocks. simpl.
+          repeat rewrite Pregmap.gso by congruence.
+          rewrite Z.add_0_r. eauto.
+        * red. intros b delta o k p. rewrite_perms. rewrite_stack_blocks. rewrite in_stack_cons.
+          intros. exploit NIB; eauto. tauto.
+        * rewrite_stack_blocks. constructor.
+          eapply inject_stack_more_perm. 2: eauto. intros. rewrite_perms. auto.
+        * red. rewrite_stack_blocks. simpl. intros b fi delta H H0 b' o delta' k p. rewrite_perms. eapply IP; eauto. tauto.
+        * rewnb. auto.
+        * rewrite_stack_blocks. simpl; auto.
+        * red. auto.
+      + (* call_r *)
+        inv EI. inv MS. do 4 eexists. split. eauto. split. econstructor; eauto.
+        * instantiate (1:= (None,nil)::lprog). simpl. eapply Mem.inject_push_new_stage_left; eauto.
+        * rewrite_stack_blocks. rewrite STK; auto. 
+        * intros; apply val_inject_set; auto.
+          intros; apply val_inject_set; auto.
+          apply Val.offset_ptr_inject; auto.
+        * red. rewrite_stack_blocks. simpl.
+          repeat rewrite Pregmap.gso by congruence.
+          rewrite Z.add_0_r. eauto.
+        * red. intros b delta o k p. rewrite_perms. rewrite_stack_blocks. rewrite in_stack_cons.
+          intros. exploit NIB; eauto. tauto.
+        * rewrite_stack_blocks. constructor. eapply inject_stack_more_perm. 2: eauto. intros; rewrite_perms; auto.
+        * red. rewrite_stack_blocks. simpl. intros b fi delta H H0 b' o delta' k p. rewrite_perms. eapply IP; eauto. tauto.
+        * rewnb. auto.
+        * rewrite_stack_blocks. simpl; auto.
+        * red. auto.
+      + (* ret *)
+        unfold Asm.exec_instr in EI. simpl in EI.
+        repeat destr_in EI.
+        eexists j,ostack, _, _; split; eauto. split; auto.
+        inv MS.
+        assert (exists f rprog, lprog = f :: rprog).
+        {
+          inv t.
+          rewrite <- H in IS.
+          destruct lprog. exfalso.
+          revert init_sp_ptr; unfold init_sp; simpl in STK; rewrite <- STK.
+          rewrite <- H. simpl. unfold current_frame_sp. rewrite H0. inversion 1.
+          eauto.
+        }
+        destruct H as (ff & rprog & EQ). subst.
+        simpl in MINJ.
+        econstructor; eauto.
+        * eapply Mem.unrecord_stack_block_inject_left_zero; eauto.
+          red. inv t. constructor. unfold in_frames; rewrite H0. easy.
+          omega.
+        * rewrite_stack_blocks.
+          rewrite STK. simpl. eauto.
+        * simpl; intros. apply val_inject_set; auto.
+          intros; apply val_inject_set; auto.
+        * red. repeat rewrite Pregmap.gso by congruence.
+          rewrite_stack_blocks. inv t. rewrite EQ in H; inv H. simpl.
+          intros; erewrite AGSP; eauto.
+          rewrite EQ. simpl. rewrite H0. simpl.  omega.
+        * red; intros. rewrite_stack_blocks. revert EQ. inv t. inversion 1; subst. simpl.
+          red in NIB. rewrite <- H1 in NIB.
+          revert H0. rewrite_perms. intro.
+          exploit NIB; eauto. rewrite in_stack_cons; unfold in_frames; rewrite H2. simpl. tauto.
+        * rewrite_stack_blocks. revert EQ. inv t. inversion 1; subst. simpl.
+          rewrite <- H in IS. inv IS.
+          eapply inject_stack_more_perm. 2: eauto. intros; rewrite_perms. auto. inv H0.
+        * red. rewrite_stack_blocks. revert EQ. inv t. inversion 1; subst. simpl.
+          red in IP. rewrite <- H in IP.
+          intros. revert H4; rewrite_perms. eapply IP; eauto.
+          right. auto.
+        * rewnb. auto.
+        * rewrite_stack_blocks. revert EQ. inv t. inversion 1; subst. rewrite <- H in SPinstack. simpl.
+          simpl in SPinstack. destruct SPinstack. red in H1. rewrite H0 in H1; easy. auto.
+
+     + (* allocframe *)
+       clear ISUNCH.
+       unfold Asm.exec_instr in EI; simpl in EI.
+       repeat destr_in EI.
+       inversion MS; subst.
+       edestruct alloc_inject as (j' & JSPEC & INCR & m4' & STORE2 & MS') ; eauto.
+       apply Ptrofs.unsigned_range_2.
+       simpl in *.
+       rewrite Ptrofs.repr_unsigned in STORE2. setoid_rewrite STORE2.
+       eexists j', _, _, _; split; eauto.
+
+     + (* freeframe *)
+       unfold Asm.exec_instr in EI; simpl in EI.
+       repeat (destr_in EI; [idtac]).
+       clear ISUNCH.
+       rename Heqv0 into RS1RSP.
+       rename Heqo into LOADRA.
+       rename Heqb0 into CHECKFRAME.
+       rename Heqo0 into FREE.
+       rename Heqo1 into UNRECORD.
+       rename Heqo2 into ISDEF.
+       inv MS. rewrite RS1RSP in RSPzero. destruct RSPzero as [bb EQ]; inv EQ.
+       exploit Mem.loadv_inject. eauto. apply LOADRA.
+       apply Val.offset_ptr_inject. rewrite <- RS1RSP; auto.
+       intros (ra' & LOADRA' & INJra).
+       rewrite LOADRA'.
+       unfold check_top_frame in CHECKFRAME.
+       repeat destr_in CHECKFRAME.
+       (* repeat destr_in AGSP1. *)
+       repeat rewrite andb_true_iff in H0.
+       destruct H0 as (A & B).
+       destruct Forall_dec; simpl in A; try congruence. clear A.
+       apply ZEQ in B.
+       set (newostack := Ptrofs.unsigned ostack0 + align ((frame_adt_size f0)) 8).
+
+       assert (RNGframe: 0 <= align (frame_adt_size f0) 8 < Ptrofs.max_unsigned).
+       {
+         generalize (size_active_stack_below m1).
+         generalize (size_active_stack_pos (Mem.stack m1)). rewrite Heqs.
+         generalize (size_active_stack_pos s).
+         generalize (Mem.stack_limit_range).
+         simpl. unfold size_frame. 
+         split. apply size_frame_pos.
+         omega.
+       }
+
+       exploit Mem.free_left_inject. apply MINJ. eauto. intro MINJ'.
+       exploit Mem.tailcall_stage_inject_left. apply MINJ'. eauto.
+       intros INJ. 
+       exists j, newostack; eexists; eexists; split; [|split]; eauto.
+       generalize (RINJ RSP). rewrite RS1RSP.
+       inversion 1 as [ff|ff|ff|ff|? ? ? ? ? INJB ? x EQRSP|ff]; subst.
+       symmetry in EQRSP.
+       rewrite Ptrofs.add_zero_l in *.
+       inversion IS. subst. rewrite BLOCKS in f1. inv f1. red in H2; simpl in H2; destruct H2 as [? _]; subst. clear H3. rewrite JB in INJB; inv INJB.
+       specialize (AGSP _ EQRSP).
+       specialize (SPAL _ EQRSP).
+       rewrite EQRSP in RSPEQ. inv RSPEQ.
+       assert (0 <= Mem.stack_limit - size_active_stack (Mem.stack m1') <= Ptrofs.max_unsigned) as RNGnewofs. 
+       {
+         generalize (size_active_stack_below m1').
+         generalize (size_active_stack_pos (Mem.stack m1')).
+         generalize (Mem.stack_limit_range).
+         omega.
+       }
+       assert (0 <= newostack <= Ptrofs.max_unsigned) as RNGnew.
+       {
+         unfold newostack.
+         rewrite AGSP. rewrite Heqs. simpl.
+         revert RNGnewofs. repeat rewrite_stack_blocks. simpl.
+         rewrite Heqs. inversion 1; subst. unfold size_frame. intros; omega.
+       }
+       rewrite <- (Ptrofs.unsigned_repr newostack) by omega.
+       destruct lprog.
+       {
+         simpl in STK.
+         revert init_sp_ptr; unfold init_sp; simpl in STK; rewrite <- STK. simpl.
+         unfold current_frame_sp. simpl. repeat destr. inv BLOCKS.
+         red in c. simpl in c.
+         revert c. unfold current_frame_sp. simpl. rewrite Heql0.
+         repeat rewrite_stack_blocks. rewrite in_stack_cons.
+         rewrite Heqs. inversion 1. subst s f1. intros [[]|INS]. inversion 1. subst b.
+         exploit Mem.stack_norepet; rewrite Heqs. clear STK. intro ND; inv ND.
+         edestruct (H4 binit_sp). red. simpl. eapply in_frame'_in_frame. red; rewrite Heql0.
+         left; reflexivity.
+         eauto.
+       }
+       eapply match_states_intro with (lprog := (None, f0::l) :: lprog ); eauto.
+       * repeat rewrite_stack_blocks. rewrite Heqs. simpl. inversion 1; subst. inv STK.
+         simpl. reflexivity.
+       * rewrite nextinstr_rsp. rewrite Pregmap.gso by congruence.
+         rewrite Pregmap.gss.
+         simpl in ISDEF. unfold is_ptr in ISDEF.
+         destr_in ISDEF. inv ISDEF. unfold current_sp, current_frame_sp in Heqv1.
+         revert Heqv1.
+         repeat destr; inversion 1. eauto.
+       * intros; apply val_inject_nextinstr.
+         intros; apply val_inject_set; auto.
+         intros; apply val_inject_set; auto.
+         assert (v0 = parent_sp (Mem.stack m1)).
+         revert ISDEF. rewrite Heqs.  simpl. unfold is_ptr. destr. 
+         simpl.
+         revert ISDEF. simpl. unfold is_ptr. destr. inversion 1; subst. inv ISDEF.
+         inv IPS_REC.
+         -- simpl in Heqv1. inv Heqv1.
+         -- simpl in Heqv1. inv Heqv1.
+         -- simpl in Heqv1. unfold current_frame_sp in Heqv1; simpl in Heqv1.
+            rewrite BLOCKS0 in Heqv1. inv Heqv1.
+            econstructor. eauto.
+            rewrite Ptrofs.add_zero_l.
+            rewrite Ptrofs.add_unsigned.
+            f_equal. setoid_rewrite Ptrofs.unsigned_repr. simpl.
+            unfold size_frame; rewrite SIZE0, SIZE.
+            rewrite Z.max_r by (apply frame_size_pos). omega.
+            generalize (size_active_stack_below m1).
+            generalize (size_active_stack_pos (Mem.stack m1)).
+            rewrite Heqs. simpl. unfold size_frame. rewrite SIZE, SIZE0.
+            generalize Mem.stack_limit_range. omega.
+            rewrite Z.max_r by apply frame_adt_size_pos. omega.
+         
+       * red. rewrite nextinstr_rsp.
+         rewrite ! Pregmap.gso by congruence.
+         rewrite Pregmap.gss. simpl. inversion 1; subst.
+         repeat rewrite_stack_blocks. rewrite Ptrofs.add_unsigned. rewrite AGSP. rewrite Heqs. simpl.
+         inversion 1. subst.
+         rewrite Z.max_r by apply frame_adt_size_pos.
+         unfold size_frame.
+         rewrite Ptrofs.unsigned_repr. 
+         rewrite Ptrofs.unsigned_repr by omega.
+         omega.
+         rewrite Ptrofs.unsigned_repr by omega.
+         generalize (size_active_stack_below m1). rewrite Heqs. simpl.
+         generalize (size_active_stack_pos r). 
+         generalize Mem.stack_limit_range.
+         unfold size_frame. omega.
+       * red. rewrite nextinstr_rsp.
+         rewrite ! Pregmap.gso by congruence.
+         rewrite Pregmap.gss. simpl. inversion 1. subst. clear H0.
+         rewrite Ptrofs.add_unsigned.
+         rewrite Ptrofs.unsigned_repr_eq. rewrite AGSP.
+         rewrite Z.max_r by apply frame_adt_size_pos.
+         rewrite Ptrofs.unsigned_repr by omega.
+
+         apply mod_divides. vm_compute. congruence. rewrite Ptrofs.modulus_power.
+         exists (two_p (Ptrofs.zwordsize - 3)). change 8 with (two_p 3). rewrite <- two_p_is_exp. f_equal. vm_compute. congruence. omega.
+         apply Z.divide_add_r.
+         apply Z.divide_sub_r.
+         apply Mem.stack_limit_aligned.
+         apply size_active_stack_divides.
+         apply align_divides. omega.
+       * rewrite nextinstr_rsp.
+         rewrite ! Pregmap.gso by congruence.
+         rewrite Pregmap.gss.
+         f_equal. unfold newostack.
+         simpl. rewrite Z.max_r. rewrite Ptrofs.add_unsigned.
+         rewrite AGSP.
+         rewrite Ptrofs.unsigned_repr by omega.
+         reflexivity.
+         apply frame_adt_size_pos.
+       * red. intros b' delta0 o k p JB0.
+         repeat rewrite_perms. destr. intro PERMS.
+         generalize (NIB b' delta0 o k p JB0 PERMS).
+         intros (LE & INS).
+         destruct (peq b b').
+         -- subst.
+            rewrite perm_stack_eq in PERMS; eauto.
+            2: rewrite Heqs; econstructor; eauto.
+            2: rewrite Heqs. 2: left. 2: red; simpl. 2: red; rewrite BLOCKS; left; reflexivity.
+            rewrite <- SIZE in PERMS.
+            apply zle_zlt in PERMS. rewrite <- andb_assoc in Heqb0. rewrite PERMS in Heqb0. inv Heqb0.
+         -- repeat rewrite_stack_blocks. rewrite Heqs. simpl. 
+            rewrite Heqs in INS.
+            rewrite in_stack_cons in INS. destruct INS.
+            red in H0. simpl in H0.
+            unfold get_frame_blocks in H0. rewrite BLOCKS in H0. simpl in H0. destruct H0;[|easy]. subst.
+            intuition.
+            rewrite in_stack_cons. split; auto.
+            rewrite Ptrofs.unsigned_repr by omega.
+            unfold newostack.
+            rewrite SIZE.
+            destruct (zle (Ptrofs.unsigned (Ptrofs.repr (Mem.stack_limit - size_active_stack s - align ((frame_size fi)) 8)) + align ((frame_size fi)) 8) (o + delta0)); auto.
+            exfalso.
+            apply Z.gt_lt in g.
+
+            rewrite AGSP in LE, g.
+            
+            assert (max_perm: forall m b o k p, Mem.perm m b o k p -> Mem.perm m b o Max Nonempty).
+            {
+              intros.
+              eapply Mem.perm_implies.
+              eapply Mem.perm_max. eauto. constructor.
+            }
+            generalize (Mem.free_range_perm _ _ _ _ _ FREE). intro FP.
+            assert (LT: 0 < frame_size fi).
+            {
+              destruct (zlt 0 (frame_size fi)); auto.
+              assert (frame_size fi = 0). generalize (frame_size_pos fi); omega.
+              rewrite H2 in g.
+              change (align 0 8) with 0 in g. omega.
+            }
+            revert LE g. rewrite Heqs.
+
+            simpl. inv H1.
+            unfold size_frame. rewrite SIZE. rewrite Z.sub_add_distr. intros.
+            set (delta := Mem.stack_limit - size_active_stack r - align ((frame_size fi)) 8) in *.
+            destruct (zlt (o + delta0) (delta + frame_size fi)).
+            ++
+              assert (DISJ: forall ofs , Mem.perm m1 b ofs Cur Freeable -> bstack <> bstack \/ o + delta0 <> ofs + delta).
+              intros; eapply Mem.mi_no_overlap. apply MINJ. apply not_eq_sym. apply n. auto. auto. eapply max_perm; eauto.
+              eapply max_perm; eauto.
+              assert (exists o2, 0 <= o2 < frame_size fi /\ o + delta0 = o2 + delta) as EX.
+              {
+                exists (o + delta0 - delta). omega.
+              }
+              destruct EX as (o2 & RNG & EQ').
+              edestruct DISJ; eauto.
+            ++ assert (delta + frame_size fi <= o + delta0 < delta + align (frame_size fi) 8).
+               omega.
+               assert (exists o2, frame_size fi <= o2 < align (frame_size fi) 8 /\ o + delta0 = o2 + delta) as EX.
+               {
+                 exists (o + delta0 - delta).
+                 omega.
+               }
+               destruct EX as (o2 & RNG & EQ').
+               eapply IP. 4: apply PERMS.  3: eauto. 2: apply JB.
+               rewrite Heqs. left. red. simpl. red; rewrite BLOCKS. left; reflexivity. omega.
+            ++ intuition congruence.
+       * repeat rewrite_stack_blocks. rewrite Heqs. simpl. inversion 1. subst. constructor.
+         eapply perm_stack_inv. eauto.
+         intros. repeat rewrite_perms. destr.
+         repeat rewrite andb_true_iff in Heqb1. destruct Heqb1 as ((A & B) & C).
+         destruct (peq b b0); simpl in *; try congruence. subst.
+         exploit Mem.stack_norepet. rewrite Heqs. intro ND; inv ND.
+         eapply H5 in H0; eauto.
+       * red. intros b0 fi0 delta' INSTK JB0 b2 o delta2 k p JB2 PERMS.
+         revert INSTK. repeat rewrite_stack_blocks. rewrite Heqs. inversion 1; subst. simpl.
+         intros [[]|INSTK].
+         eapply IP with (k:= k) (p:=p); eauto. rewrite Heqs. simpl. right; eauto. 
+         revert PERMS. repeat rewrite_perms. destr.
+       * rewnb. xomega.
+       * repeat rewrite_stack_blocks. rewrite Heqs. simpl. auto.
+         inversion 1; subst.
+         simpl in SPinstack. unfold current_frame_sp in SPinstack. simpl in SPinstack.
+         destruct SPinstack; auto.
+         simpl.  right. red in H0. simpl in H0. red in H0. rewrite BLOCKS in H0.
+         destruct H0 as [IFR|[]]. inv IFR.
+         red in c.
+         revert c. rewrite EQ2.
+         unfold Asm.init_sp.
+         revert init_sp_ptr. unfold init_sp. intro A; rewrite A.
+         rewrite in_stack_cons. intros [[]|INS]. 
+         exploit Mem.stack_norepet. rewrite Heqs. intro ND; exfalso; inv ND.
+         apply (H3 binit_sp).
+         red; simpl. eapply in_frame'_in_frame; eauto. red; rewrite BLOCKS; left; eauto.
+         auto.
+
+     + (* load parent pointer *)
+       unfold Asm.exec_instr in EI; simpl in EI.
+       unfold check_top_frame in EI.
+       destruct (Mem.stack m1) eqn:S1; try congruence.
+       repeat destr_in EI.
+       repeat destr_in Heqb.
+       apply andb_true_iff in H0; destruct H0 as (A & B).
+       apply ZEQ in B. subst.
+       destruct Forall_dec; simpl in A; try congruence. clear A.
+       assert (RNGframe: 0 <= align (frame_adt_size f0) 8 < Ptrofs.max_unsigned).
+       {
+         generalize (size_active_stack_below m1').
+         generalize (size_active_stack_pos (Mem.stack m1')). rewrite S1.
+         generalize (Mem.stack_limit_range).
+         generalize (frame_adt_size_pos f0) (align_le (frame_adt_size f0) 8) (size_stack_pos s).
+         generalize (size_active_stack_pos s).
+         simpl. unfold size_frame.
+         split. omega. omega.
+       }
+       exists j, ostack; eexists; eexists; split. eauto.
+       split; auto.
+       inversion MS; subst; econstructor; eauto.
+       * rewrite nextinstr_rsp.
+         destruct (preg_eq RSP rd).
+         rewrite e. rewrite Pregmap.gss. congruence.
+         rewrite Pregmap.gso. eauto. auto.
+       * intros; apply val_inject_nextinstr.
+         intros; apply val_inject_set; auto. rewrite S1 in *.
+         simpl in Heqo.
+         unfold is_ptr in Heqo; destr_in Heqo. inv Heqo.
+         inv IS. 
+         rewrite <- Heqv0. unfold current_sp. destr. inv Heqv0.
+         inv IPS_REC. inv Heqv0. simpl in *.
+         repeat destr_in Heqv0. inv BLOCKS0.
+         rewrite RSPEQ. simpl.
+         unfold current_frame_sp. simpl. rewrite H2.
+         econstructor; eauto. rewrite Ptrofs.add_zero_l.
+         rewrite Ptrofs.add_unsigned. 
+         rewrite AGSP. rewrite S1.
+         simpl. simpl. unfold size_frame.
+         rewrite <- SIZE0.
+         repeat rewrite Z.max_r by (apply frame_adt_size_pos). f_equal.
+         rewrite Ptrofs.unsigned_repr.
+         omega. omega.
+         auto.
+       * red. rewrite nextinstr_rsp.
+         rewrite Pregmap.gso; eauto.
+       * red. rewrite nextinstr_rsp.
+         rewrite Pregmap.gso; eauto.
+       * rewrite nextinstr_rsp.
+         rewrite Pregmap.gso; eauto.
+  Qed.
+
+  Definition asm_prog_no_rsp (ge: Genv.t Asm.fundef unit):=
+    forall b f,
+      Genv.find_funct_ptr ge b = Some (Internal f) ->
+      asm_code_no_rsp (fn_code f).
+
+  Hypothesis prog_no_rsp: asm_prog_no_rsp ge.
+
+  Context `{ecprops: !ExternalCallsProps mem}.
+
+  Lemma inj_incr_sep_same:
+    forall j j' m1 m2 b1 b2 delta,
+      inject_incr j j' ->
+      inject_separated j j' m1 m2 ->
+      j' b1 = Some (b2, delta) ->
+      Mem.valid_block m2 b2 ->
+      j b1 = Some (b2, delta).
+  Proof.
+    intros.
+    destruct (j b1) eqn:JB.
+    destruct p. eapply H in JB; eauto.
+    congruence.
+    exploit H0; eauto. intuition congruence.
+  Qed.
+
+  Lemma set_res_no_rsp:
+    forall res vres rs,
+      no_rsp_builtin_preg res ->
+      set_res res vres rs RSP = rs RSP.
+  Proof.
+    induction res; simpl.
+    - intros. eapply Pregmap.gso. auto.
+    - auto.
+    - intros vres rs (NR1 & NR2).
+      rewrite IHres2; auto.
+  Qed.
+
+  Lemma val_inject_set_res:
+    forall r rs1 rs2 v1 v2 j,
+      Val.inject j v1 v2 ->
+      (forall r0, Val.inject j (rs1 r0) (rs2 r0)) ->
+      forall r0, Val.inject j (set_res r v1 rs1 r0) (set_res r v2 rs2 r0).
+  Proof.
+    induction r; simpl; intros; auto.
+    apply val_inject_set; auto.
+    eapply IHr2; eauto.
+    apply Val.loword_inject. auto.
+    intros; eapply IHr1; eauto.
+    apply Val.hiword_inject. auto.
+  Qed.
+
+  Definition init_data_diff (id: init_data) (i: ident) :=
+    match id with
+      Init_addrof ii _ => ii <> i
+    | _ => True
+    end.
+
+  Lemma store_init_data_eq:
+    forall F V m (ge: _ F V) id gv b o i,
+      init_data_diff i id ->
+      Genv.store_init_data (Genv.add_global ge (id,gv)) m b o i =
+      Genv.store_init_data ge m b o i.
+  Proof.
+    destruct i; simpl; intros; auto.
+    unfold Genv.find_symbol; simpl. 
+    rewrite Maps.PTree.gso; auto.
+  Qed.
+
+  Lemma store_init_data_list_eq:
+    forall F V id i, 
+      Forall (fun x => init_data_diff x id) i ->
+      forall m (ge: _ F V) gv b o,
+        Genv.store_init_data_list (Genv.add_global ge (id,gv)) m b o i =
+        Genv.store_init_data_list ge m b o i.
+  Proof.
+    induction 1; simpl; intros; auto.
+    rewrite store_init_data_eq; auto.
+    destr. 
+  Qed.
+
+  Lemma alloc_global_eq:
+    forall F V (l: (ident * option (globdef F V))) m (ge: _ F V) id gv,
+      (forall v, snd l = Some (Gvar v) -> Forall (fun x => init_data_diff x id) (gvar_init v)) ->
+      Genv.alloc_global (Genv.add_global ge (id,gv)) m l =
+      Genv.alloc_global ge m l .
+  Proof.
+    destruct l; simpl; intros.
+    repeat (destr; [idtac]).
+    rewrite store_init_data_list_eq. auto.
+    apply H; auto.
+  Qed.
+
+  Lemma alloc_globals_eq:
+    forall F V (l: list (ident * option (globdef F V))) m (ge: _ F V) id gv,
+      (forall x v, In x l -> snd x = Some (Gvar v) -> Forall (fun x => init_data_diff x id) (gvar_init v)) ->
+      Genv.alloc_globals (Genv.add_global ge (id,gv)) m l =
+      Genv.alloc_globals ge m l .
+  Proof.
+    induction l; simpl; intros; eauto.
+    rewrite alloc_global_eq. destr.
+    apply IHl. intros; eauto.
+    eauto.
+  Qed.
+
+  Lemma find_symbol_add_globals_other:
+    forall F V l (ge: _ F V) s,
+      ~ In s (map fst l) ->
+      Genv.find_symbol (Genv.add_globals ge l) s =
+      Genv.find_symbol ge s.
+  Proof.
+    induction l; simpl; intros; eauto.
+    rewrite IHl.
+    unfold Genv.find_symbol; simpl.
+    apply Maps.PTree.gso. intuition. intuition.
+  Qed.
+
+
+  Lemma find_symbol_add_global_other:
+    forall F V l (ge: _ F V) s,
+      s <> fst l ->
+      Genv.find_symbol (Genv.add_global ge l) s =
+      Genv.find_symbol ge s.
+  Proof.
+    destruct l; simpl; intros; eauto.
+    unfold Genv.find_symbol; simpl.
+    apply Maps.PTree.gso. intuition. 
+  Qed.
+
+  Lemma find_symbol_none_add_global:
+    forall F V (ge: Genv.t F V) a i,
+      Genv.find_symbol (Genv.add_global ge a) i = None ->
+      i <> fst a /\ Genv.find_symbol ge i = None.
+  Proof.
+    unfold Genv.find_symbol; simpl.
+    intros F V ge0 a i.
+    rewrite Maps.PTree.gsspec.
+    destr.
+  Qed.
+
+  Lemma find_symbol_none_add_globals:
+    forall F V a (ge: Genv.t F V) i,
+      Genv.find_symbol (Genv.add_globals ge a) i = None ->
+      ~ In i (map fst a) /\ Genv.find_symbol ge i = None.
+  Proof.
+    induction a; simpl; intros; eauto.
+    apply IHa in H.
+    destruct H as (H1 & H).
+    apply find_symbol_none_add_global in H; auto.
+    intuition.
+  Qed.
+
+  Lemma find_symbol_none_not_in_defs:
+    forall F V (p: program F V) i,
+      Genv.find_symbol (Genv.globalenv p) i = None ->
+      ~ In i (map fst (prog_defs p)).
+  Proof.
+    unfold Genv.globalenv.
+    intros F V p.
+    generalize (Genv.empty_genv F V (prog_public p)).
+    generalize (prog_defs p).
+    induction l; simpl; intros; eauto.
+    apply find_symbol_none_add_globals in H.
+    destruct H as (A & B).
+    apply find_symbol_none_add_global in B.
+    destruct B as (B & C).
+    intuition.    
+  Qed.
+
+  Lemma extcall_arg_inject:
+    forall j g rs1 m1 arg1 loc rs2 m2,
+      extcall_arg rs1 m1 loc arg1 ->
+      (forall r, Val.inject j (rs1 r) (rs2 r)) ->
+      Mem.inject j g m1 m2 ->
+      exists arg2,
+        extcall_arg rs2 m2 loc arg2 /\
+        Val.inject j arg1 arg2.
+  Proof.
+    destruct 1; simpl; intros.
+    eexists; split; try econstructor; eauto.
+    exploit Mem.loadv_inject; eauto.
+    apply Val.offset_ptr_inject; eauto.
+    intros (v2 & LOAD & INJ).
+    eexists; split; try econstructor; eauto.
+  Qed.
+
+  Lemma extcall_arg_pair_inject:
+    forall j g rs1 m1 arg1 ty rs2 m2,
+      extcall_arg_pair rs1 m1 ty arg1 ->
+      (forall r, Val.inject j (rs1 r) (rs2 r)) ->
+      Mem.inject j g m1 m2 ->
+      exists arg2,
+        extcall_arg_pair rs2 m2 ty arg2 /\
+        Val.inject j arg1 arg2.
+  Proof.
+    destruct 1; simpl; intros.
+    eapply extcall_arg_inject in H; eauto.
+    destruct H as (arg2 & EA & INJ);
+      eexists; split; try econstructor; eauto.
+    eapply extcall_arg_inject in H; eauto.
+    destruct H as (arg2 & EA & INJ).
+    eapply extcall_arg_inject in H0; eauto.
+    destruct H0 as (arg3 & EA1 & INJ1).
+    eexists; split; try econstructor; eauto.
+    apply Val.longofwords_inject; eauto.
+  Qed.
+
+  Lemma extcall_arguments_inject:
+    forall j g rs1 m1 args1 sg rs2 m2,
+      extcall_arguments rs1 m1 sg args1 ->
+      (forall r, Val.inject j (rs1 r) (rs2 r)) ->
+      Mem.inject j g m1 m2 ->
+      exists args2,
+        extcall_arguments rs2 m2 sg args2 /\
+        Val.inject_list j args1 args2.
+  Proof.
+    unfold extcall_arguments.
+    intros j g rs1 m1 args1 sg rs2 m2.
+    revert args1. generalize (loc_arguments sg).
+    induction 1; simpl; intros; eauto.
+    exists nil; split; try econstructor.
+    eapply extcall_arg_pair_inject in H; eauto.
+    decompose [ex and] H.
+    edestruct IHlist_forall2 as (a2 & EA & INJ); eauto.
+    eexists; split; econstructor; eauto.
+  Qed.
+
+  Lemma set_pair_no_rsp:
+    forall p res rs,
+      no_rsp_pair p ->
+      set_pair p res rs RSP = rs RSP.
+  Proof.
+    destruct p; simpl; intros; rewrite ! Pregmap.gso; intuition. 
+  Qed.
+
+  Lemma val_inject_set_pair:
+    forall j p res1 res2 rs1 rs2,
+      (forall r, Val.inject j (rs1 r) (rs2 r)) ->
+      Val.inject j res1 res2 ->
+      forall r,
+        Val.inject j (set_pair p res1 rs1 r) (set_pair p res2 rs2 r).
+  Proof.
+    destruct p; simpl; intros; eauto.
+    apply val_inject_set; auto.
+    repeat (intros; apply val_inject_set; auto).
+    apply Val.hiword_inject; auto.
+    apply Val.loword_inject; auto.
+  Qed.
+
+  Theorem step_simulation:
+    forall S1 t S2,
+      Asm.step init_stk ge S1 t S2 ->
+      forall j ostack S1' (MS: match_states j ostack S1 S1'),
+      exists j' ostack' S2',
+        step ge S1' t S2' /\
+        match_states j' ostack' S2 S2'.
+  Proof.
+    destruct 1; intros; inversion MS; subst.
+    - (* internal step *)
+      generalize (RINJ PC); rewrite H. inversion 1; subst.
+      assert (j b = Some (b,0)) as JB.
+      {
+        eapply GLOBFUN_INJ. eauto.
+      }
+      rewrite JB in H7; inv H7. 
+      assert (asm_instr_no_rsp i).
+      {
+        eapply prog_no_rsp. eauto.
+        eapply Asmgenproof0.find_instr_in; eauto.
+      }
+      destruct (exec_instr_inject' _ _ _ _ _ _ _ _ _ _ MS H4 (asmgen_no_change_stack i) H2)
+        as ( j' & ostack' & rs2' & m2' & EI' & MS' & INCR).
+      do 3 eexists; split.
+      eapply exec_step_internal; eauto.
+      rewrite Ptrofs.add_zero. eauto.
+      eauto.
+    - (* builtin step *)
+      edestruct (eval_builtin_args_inject) as (vargs' & Hargs & Hargsinj).
+      6: eauto.
+      eauto. eauto. eauto.
+      eauto. 
+      eapply GLOBSYMB_INJ.
+      edestruct (external_call_mem_inject_gen ef ge ge)
+        as (j' & vres' & m2' & EC & RESinj & MemInj & Unch1 & Unch2 & INCR & SEP).
+      apply meminj_preserves_globals'_symbols_inject.
+      eauto.
+      eauto.
+      eapply Mem.inject_push_new_stage_left. eauto.
+      eauto.
+      assert (j b = Some (b,0)) as JB.
+      {
+        eapply GLOBFUN_INJ. eauto.
+      }
+      generalize (RINJ PC); rewrite H. inversion 1; subst.
+      rewrite JB in H10; inv H10.
+      exploit Mem.unrecord_stack_block_inject_left. apply MemInj. eauto.
+      omega. 
+      red; repeat rewrite_stack_blocks. constructor. easy. 
+      intro MemInj'.
+      do 3 eexists; split.
+      eapply exec_step_builtin.
+      eauto.
+      eauto. 
+      rewrite Ptrofs.add_zero; eauto.
+      eauto.
+      eauto.
+      auto.
+      reflexivity.
+      econstructor.
+      + eauto.
+      + repeat rewrite_stack_blocks. simpl; eauto.
+      + reflexivity.
+      + rewrite nextinstr_nf_rsp.
+        rewrite set_res_no_rsp.
+        rewrite Asmgenproof0.undef_regs_other.
+        eauto.
+        intros; intro; subst. rewrite in_map_iff in H7.
+        destruct H7 as (x & EQ & IN).
+        apply preg_of_not_rsp in EQ. congruence.
+        auto.
+      + intros. apply val_inject_nextinstr_nf.
+        apply val_inject_set_res; auto.
+        apply val_inject_undef_regs; auto.
+        intros; eapply val_inject_incr; eauto.
+      + red; rewnb. auto.
+      + red. rewrite nextinstr_nf_rsp.
+        rewrite set_res_no_rsp; auto.
+        rewrite Asmgenproof0.undef_regs_other.
+        repeat rewrite_stack_blocks. simpl; auto.
+        intros r INR EQ; subst.
+        rewrite in_map_iff in INR.
+        destruct INR as (x & EQ & IN).
+        apply preg_of_not_rsp in EQ. congruence.
+      (* + red. erewrite <- external_call_stack_blocks. 2: eauto. *)
+      (*   rewrite nextinstr_nf_rsp. *)
+      (*   rewrite set_res_no_rsp; auto. *)
+      (*   rewrite Asmgenproof0.undef_regs_other. eauto. *)
+      (*   intros; intro; subst. *)
+      (*   rewrite in_map_iff in H6. *)
+      (*   destruct H6 as (x & EQ & IN). *)
+      (*   apply preg_of_not_rsp in EQ. congruence. *)
+      (* + erewrite <- external_call_stack_blocks; eauto. *)
+      + red. 
+        rewrite nextinstr_nf_rsp.
+        rewrite set_res_no_rsp; auto.
+        rewrite Asmgenproof0.undef_regs_other. eauto.
+        intros r' INR; intro; subst.
+        rewrite in_map_iff in INR.
+        destruct INR as (x & EQ & IN).
+        apply preg_of_not_rsp in EQ. congruence.
+      + red. intros ofs0 k p PERM.
+        revert PERM; rewrite_perms. eauto.
+        destruct NS as (fr & fi & r & STK' & BLK & ZERO & PUB).
+        rewrite STK'.
+        rewrite in_stack_cons; left. 
+        rewrite in_frames_cons. eexists; split; eauto.
+        red; unfold get_frame_blocks; rewrite <- BLK. simpl. auto.
+      + red.
+        intros.
+        eapply ec_perm_unchanged. eapply external_call_spec. eauto.
+        eauto.
+        intros. eapply PBS in H8. destruct H8.  intro A; inv A; inv H10. 
+        eauto.
+      + red.
+        erewrite <- external_call_stack_blocks. 2: eauto.
+        eauto.
+      + rewrite nextinstr_nf_rsp.
+        rewrite set_res_no_rsp; auto.
+        rewrite Asmgenproof0.undef_regs_other. eauto.
+        intros ? INR; intro; subst.
+        rewrite in_map_iff in INR.
+        destruct INR as (x & EQ & IN).
+        apply preg_of_not_rsp in EQ. congruence.
+      + red. intros b delta o k p JB1 PERM.
+        repeat rewrite_stack_blocks. simpl.
+        destruct (j b) eqn:A. destruct p0.
+        exploit INCR. eauto. eauto. intro JB2. rewrite JB1 in JB2; inv JB2.
+        eapply NIB; eauto.
+        eapply Mem.perm_max in PERM. eapply Mem.push_new_stage_perm.
+        eapply external_call_max_perm. eauto. red; rewnb.
+        eapply Mem.valid_block_inject_1; eauto.
+        eapply Mem.unrecord_stack_block_perm. eauto. eauto.
+        exploit SEP. eauto. eauto.
+        unfold Mem.valid_block.  rewnb. intuition congruence. 
+      + eapply inject_stack_incr. apply INCR.
+        repeat rewrite_stack_blocks. simpl.
+        eapply perm_stack_inv. eauto. intros.
+        repeat rewrite_perms; auto. rewrite_stack_blocks. rewrite in_stack_cons; auto.
+      + red.
+        repeat rewrite_stack_blocks. simpl.
+        intros b fi delta INS J'B b' o delta' k p J'B' PERM.
+        exploit inj_incr_sep_same. eauto. eauto. apply J'B. auto.
+        exploit inj_incr_sep_same. eauto. eauto. apply J'B'. auto.
+        intros NJB' NJB.
+        eapply IP; eauto.
+        eapply Mem.perm_max in PERM. eapply Mem.push_new_stage_perm.
+        eapply external_call_max_perm. eauto. red; rewnb.
+        eapply Mem.valid_block_inject_1; eauto.
+        eapply Mem.unrecord_stack_block_perm. eauto. eauto.
+      + intros.
+        eapply INCR; eauto.
+      + intros.
+        eapply INCR; eauto.
+      + destruct GLOBSYMB_INJ.
+        split. intros.
+        eapply INCR; eauto.
+        intros.
+        destruct (j b1) eqn:JB1.
+        destruct p.
+        exploit INCR; eauto. rewrite H10; intro X; inv X.
+        eauto.
+        exploit SEP; eauto. unfold Mem.valid_block; rewnb. intros (NV1 & NV2).
+        simpl; unfold Genv.block_is_volatile.
+        rewrite ! find_var_info_none_ge.
+        auto.
+        unfold Mem.valid_block in NV1. xomega.
+        unfold Mem.valid_block in NV2. xomega.
+      + etransitivity. apply GlobLe. fold Ple. rewnb. xomega.
+      + etransitivity. apply GlobLeT. fold Ple. rewnb. xomega.
+      + repeat rewrite_stack_blocks. simpl; eauto.
+    - (* external step *)
+      edestruct (extcall_arguments_inject) as (vargs' & Hargs & Hargsinj).
+      eauto.
+      eauto. eauto. 
+      edestruct (external_call_mem_inject_gen ef ge ge)
+        as (j' & vres' & m2' & EC & RESinj & MemInj & Unch1 & Unch2 & INCR & SEP).
+      apply meminj_preserves_globals'_symbols_inject. eauto.
+      eauto.
+      eauto.
+      eauto. 
+      generalize (RINJ PC); rewrite H. inversion 1; subst.
+      assert (j b = Some (b,0)) as JB.
+      {
+        eapply GLOBFUN_INJ. eauto.
+      }
+      rewrite JB in H9; inv H9.
+      exploit (Mem.unrecord_stack_block_inject_left _ _ _ _ _ _ MemInj H3).
+      inv TIN. rewrite STK in H6.
+      destruct lprog; simpl in *. 2: omega.
+      revert init_sp_ptr. unfold init_sp. rewrite <- H6. simpl. unfold current_frame_sp; rewrite H7. inversion 1.
+      red; repeat rewrite_stack_blocks. inv TIN. constructor. unfold in_frames; rewrite H7. easy.
+      intro MemInj'.
+      do 3 eexists; split.
+      eapply exec_step_external.
+      eauto.
+      eauto.
+      eauto.
+      generalize (RINJ RSP). destruct (rs RSP); simpl in *; inversion 1; subst; try congruence.
+      generalize (RINJ RA). destruct (rs RA); simpl in *; inversion 1; subst; try congruence.
+      destruct Tptr; try easy.
+      destruct Tptr; try easy.
+      destruct Tptr; try easy.
+      destruct Tptr; try easy.
+      generalize (RINJ RSP). destruct (rs RSP); simpl in *; inversion 1; subst; try congruence.
+      generalize (RINJ RA). destruct (rs RA); simpl in *; inversion 1; subst; try congruence.
+      eauto.
+      reflexivity.
+
+      econstructor; eauto.
+      + repeat rewrite_stack_blocks.
+        instantiate (1 := tl lprog).
+        destruct lprog. inv TIN. exfalso.
+        revert init_sp_ptr; unfold init_sp; simpl in STK; rewrite <- STK. rewrite <- H6.
+        simpl; unfold current_frame_sp; simpl. rewrite H7; 
+        inversion 1.
+        revert EQ; rewrite_stack_blocks. intro A; rewrite A. simpl.
+        rewrite STK in A. simpl in A ; inv A. auto.
+      + destruct lprog; simpl; try reflexivity.
+        exfalso.
+        revert init_sp_ptr; unfold init_sp; simpl in STK; rewrite <- STK. rewrite STK.
+        inv TIN. rewrite <- H6.
+        simpl; unfold current_frame_sp; simpl. rewrite H7; 
+        inversion 1.        
+      + repeat rewrite Pregmap.gso by (congruence). 
+        rewrite set_pair_no_rsp.
+        rewrite Asmgenproof0.undef_regs_other.
+        rewrite Asmgenproof0.undef_regs_other.
+        eauto.
+        intros ? INR; intro; subst. rewrite in_map_iff in INR.
+        destruct INR as (x & EQ & IN).
+        apply preg_of_not_rsp in EQ. congruence.
+        intros; intro; subst. clear - H6; simpl in *; intuition congruence.
+        auto.
+      + intros; apply val_inject_set.
+        intros; apply val_inject_set.
+        intros; apply val_inject_set_pair; auto.
+        apply val_inject_undef_regs; auto.
+        apply val_inject_undef_regs; auto.
+        intros; eapply val_inject_incr; eauto.
+        intros; eapply val_inject_incr; eauto.
+        auto.
+      + red; rewnb; eauto.
+      + red. repeat rewrite Pregmap.gso by (congruence). 
+        rewrite set_pair_no_rsp.
+        rewrite Asmgenproof0.undef_regs_other.
+        rewrite Asmgenproof0.undef_regs_other.
+        repeat rewrite_stack_blocks. inv TIN. simpl.
+        intros ostack RRSP. apply AGSP in RRSP. rewrite <- H6 in RRSP. simpl in RRSP.
+        rewrite H7 in RRSP; simpl in RRSP. omega. 
+        intros ? INR; intro; subst. rewrite in_map_iff in INR.
+        destruct INR as (x & EQ & IN).
+        apply preg_of_not_rsp in EQ. congruence.
+        intros; intro; subst. clear - H6; simpl in *; intuition congruence.
+        auto.
+      + red.
+        repeat rewrite Pregmap.gso by (congruence). 
+        rewrite set_pair_no_rsp.
+        rewrite Asmgenproof0.undef_regs_other.
+        rewrite Asmgenproof0.undef_regs_other.
+        eauto.
+        intros ? INR; intro; subst. rewrite in_map_iff in INR.
+        destruct INR as (x & EQ & IN).
+        apply preg_of_not_rsp in EQ. congruence.
+        intros; intro; subst. clear - H6; simpl in *; intuition congruence.
+        auto.
+      + red.
+        intros.
+        eapply Mem.perm_max in H6.
+        eapply external_call_max_perm in H6.
+        2: eauto.
+        eauto. eauto.
+      + red.
+        intros.
+        eapply ec_perm_unchanged. eapply external_call_spec. eauto.
+        eauto.
+        intros. eapply PBS in H7. destruct H7.  intro A; inv A; inv H9.
+        eauto.
+      + red.
+        erewrite <- external_call_stack_blocks. 2: eauto.
+        eauto.
+      + repeat rewrite Pregmap.gso by (congruence). 
+        rewrite set_pair_no_rsp.
+        rewrite Asmgenproof0.undef_regs_other.
+        rewrite Asmgenproof0.undef_regs_other.
+        eauto.
+        intros ? INR; intro; subst. rewrite in_map_iff in INR.
+        destruct INR as (x & EQ & IN).
+        apply preg_of_not_rsp in EQ. congruence.
+        intros; intro; subst. clear - H6; simpl in *; intuition congruence.
+        auto. 
+      + red. intros b delta o k p JB1 PERM.
+        repeat rewrite_stack_blocks. inv TIN. simpl.
+        destruct (j b) eqn:A. destruct p0.
+        * exploit INCR. eauto. eauto. intro JB2. rewrite JB1 in JB2; inv JB2.
+          exploit NIB; eauto.
+          eapply Mem.perm_max in PERM.
+          eapply external_call_max_perm. eauto.
+          eapply Mem.valid_block_inject_1; eauto.
+          eapply Mem.unrecord_stack_block_perm; eauto. rewrite <- H6. rewrite in_stack_cons.
+          unfold in_frames; rewrite H7. intuition.
+        * exploit SEP. eauto. eauto. intuition congruence.
+      + eapply inject_stack_incr; eauto.
+        repeat rewrite_stack_blocks. inv IS. constructor. simpl.
+        eapply perm_stack_inv. eauto.
+        intros; repeat rewrite_perms; auto.
+        rewrite <- H7. rewrite in_stack_cons; auto.
+        simpl.
+        eapply perm_stack_inv. eauto.
+        intros; repeat rewrite_perms; auto.
+        rewrite <- H7. rewrite in_stack_cons; auto.
+      + red.
+        repeat rewrite_stack_blocks.
+        intros b fi delta INS J'B b' o delta' k p J'B' PERM.
+        exploit inj_incr_sep_same. eauto. eauto. apply J'B. auto.
+        exploit inj_incr_sep_same. eauto. eauto. apply J'B'. auto.
+        intros.
+        eapply IP; eauto.
+        revert INS. inv TIN. simpl. auto.
+        eapply Mem.perm_max in PERM.
+        eapply external_call_max_perm. eauto.
+        eapply Mem.valid_block_inject_1; eauto.
+        eapply Mem.unrecord_stack_block_perm; eauto.
+      + destruct GLOBSYMB_INJ.
+        split. intros.
+        eapply INCR; eauto.
+        intros.
+        destruct (j b1) eqn:JB1.
+        destruct p.
+        exploit INCR; eauto. rewrite H9; intro X; inv X.
+        eauto.
+        exploit SEP; eauto. intros (NV1 & NV2).
+        simpl; unfold Genv.block_is_volatile.
+        rewrite ! find_var_info_none_ge.
+        auto.
+        unfold Mem.valid_block in NV1. xomega.
+        unfold Mem.valid_block in NV2.
+        xomega. 
+      + etransitivity. apply GlobLe. fold Ple; rewnb; xomega.
+      + etransitivity. apply GlobLeT. fold Ple; rewnb; xomega.
+      + repeat rewrite_stack_blocks. revert SPinstack. inv TIN. simpl.
+        unfold in_frames'. rewrite H7. tauto.
+  Qed.
+
+End PRESERVATION.
+
+
+  Lemma repr_stack_limit:
+    Ptrofs.unsigned (Ptrofs.repr (Mem.stack_limit)) = Mem.stack_limit.
+  Proof.
+    apply Ptrofs.unsigned_repr.
+    generalize (Mem.stack_limit_range); omega.
+  Qed.
+  
+  Lemma match_initial_states s:
+    Asm.initial_state prog s ->
+    exists s' j ostack, match_states ((Some (make_singleton_frame_adt (Genv.genv_next ge) 0 0),nil) :: nil) (Genv.genv_next ge) j ostack s s' /\
+                   RawAsm.initial_state prog (Pregmap.init Vundef) s'.
+  Proof.
+    inversion 1. subst.
+    rename H into INIT.
+    rename H0 into INITMEM.
+    unfold Mem.record_init_sp in H1; destr_in H1.
+    rename Heqp into ALLOC.
+    rename H1 into RSB.
+    exploit Genv.initmem_inject; eauto. intro FLATINJ.
+    apply Mem.push_new_stage_inject_flat in FLATINJ.
+    assert  (ALLOCINJ:
+               exists (f' : meminj) (m2' : mem) (b2 : block),
+                 Mem.alloc (Mem.push_new_stage m0) 0 Mem.stack_limit = (m2', b2) /\
+                 Mem.inject f' (flat_frameinj (length (Mem.stack (Mem.push_new_stage m0)))) m m2' /\
+                 inject_incr (Mem.flat_inj (Mem.nextblock m0)) f' /\
+                 f' b = Some (b2, Mem.stack_limit) /\ (forall b0 : block, b0 <> b -> f' b0 = Mem.flat_inj (Mem.nextblock m2) b0)).
+    {
+      destruct (Mem.alloc (Mem.push_new_stage m0) 0 Mem.stack_limit) as (m2' & b2) eqn: ALLOC'.
+      eapply Mem.alloc_right_inject in FLATINJ; eauto.
+      exploit (Mem.alloc_left_mapped_inject _ _ _ _ _ _ _ _ b2 Mem.stack_limit FLATINJ ALLOC).
+      - exploit Mem.alloc_result; eauto. intro; subst. red; rewnb. xomega.
+      - apply Mem.stack_limit_range.
+      - intros ofs k p. rewrite_perms. rewrite pred_dec_true; auto.
+        generalize (Mem.stack_limit_range). intros; omega.
+      - intros ofs k p. omega.
+      - red. intro. generalize (size_chunk_pos chunk); omega.
+      - unfold Mem.flat_inj. intros b0 delta' ofs k p. destr. inversion 1; subst.
+        exploit Mem.alloc_result; eauto. intro; subst. xomega.
+      - repeat rewrite_stack_blocks. simpl. intuition easy.
+      - intros (f' & INJ & INCR & FB & FOTHER).
+        do 3 eexists. split; eauto. split; eauto. split; eauto. split; eauto.
+        intros; rewrite FOTHER; auto.
+        unfold Mem.flat_inj. exploit Mem.alloc_result; eauto. intro; subst.
+        revert FB FOTHER. rewnb. repeat destr. intros; xomega.
+        apply Plt_succ_inv in p. intuition. subst. contradict H. exploit Mem.alloc_result. apply ALLOC. intro; subst.
+        rewnb. auto.
+    }
+    destruct ALLOCINJ as (f' & m2' & b2 & ALLOC' & ALLOCINJ & INCR & F'B & F'O).
+    assert (b = b2).
+    {
+      exploit Mem.alloc_result. apply ALLOC.
+      exploit Mem.alloc_result. apply ALLOC'. intros; subst. rewnb. congruence.
+    }
+    subst.
+    assert (b2 = bstack).
+    {
+      unfold bstack.
+      exploit Mem.alloc_result; eauto. intro; subst.
+      rewnb. fold ge; reflexivity.
+    } subst.
+    edestruct (Mem.range_perm_drop_2) with (p := Writable) as (m3' & DROP).
+    red; intros; eapply Mem.perm_alloc_2; eauto.
+    assert (DROPINJ: Mem.inject f' (flat_frameinj (length (Mem.stack (Mem.push_new_stage m0)))) m m3').
+    {
+      eapply Mem.drop_outside_inject. apply ALLOCINJ. eauto.
+      intros b' delta ofs k p FB1 PERM RNG.
+      revert PERM; repeat rewrite_perms. destr. omega. intros.
+      revert FB1; unfold Mem.flat_inj. rewrite F'O. unfold Mem.flat_inj. destr. auto.
+    }
+    assert (RSB': exists m4',
+               Mem.record_stack_blocks m3' (make_singleton_frame_adt' bstack frame_info_mono 0) = Some m4' /\
+               Mem.inject f'
+                          (flat_frameinj (length (Mem.stack (Mem.push_new_stage m0)))) m2 m4').
+    {
+      edestruct Mem.record_stack_blocks_inject_parallel as (m4' & RSB' & RSBinj).
+      apply DROPINJ. 7: eauto.
+      instantiate (1 := make_singleton_frame_adt' bstack frame_info_mono 0).
+      - red; intros.
+        constructor; auto.
+        simpl. rewrite F'B. inversion 1.
+        eexists; split; eauto.
+        split; simpl; intros; rewrite Z.max_r in H0; omega.
+      - repeat rewrite_stack_blocks. easy.
+      - red. intros b [A|[]].
+        subst. unfold bstack; simpl.
+        red. rewnb. fold ge. xomega.
+      - intros b fi o k p [A|[]]; inv A.
+        repeat rewrite_perms. destr.
+      - unfold Mem.flat_inj. intros b1 b0 delta FB.
+        destruct (peq b1 bstack); subst. rewrite F'B in FB; inv FB. tauto.
+        rewrite F'O in FB; auto. unfold Mem.flat_inj in FB. destr_in FB. inv FB.
+        tauto.
+      - reflexivity.
+      - repeat rewrite_stack_blocks. constructor. reflexivity.
+      - repeat rewrite_stack_blocks. simpl. omega.
+      - eexists; split; eauto.
+    }
+    destruct RSB' as (m4' & RSB' & RSBINJ).
+    eexists _, f', _; split.
+    2: now (econstructor; eauto; econstructor; eauto).
+    econstructor; eauto.
+    - apply Mem.inject_push_new_stage_left.
+      revert RSBINJ.
+      instantiate (1 := (None,nil) :: nil).
+      repeat rewrite_stack_blocks. simpl. auto.
+    - repeat rewrite_stack_blocks. simpl. unfold bstack. inversion 1. intros;reflexivity.
+    - unfold rs0. rewrite Pregmap.gss. eauto.
+    - intros. unfold rs0.
+      repeat (intros; apply val_inject_set; auto).
+      + unfold ge0. unfold Genv.symbol_address. destr; auto.
+        eapply Genv.genv_symb_range in Heqo.
+        econstructor; eauto.
+        rewrite F'O.
+        unfold Mem.flat_inj. rewrite pred_dec_true. eauto. rewnb. xomega.
+        exploit Mem.alloc_result; eauto. intro; subst. rewrite H1. rewnb. apply Plt_ne. auto.
+        reflexivity.
+      + unfold Vnullptr; constructor.
+      + econstructor. rewnb. eauto. rewrite Ptrofs.add_zero_l. auto.
+    - red; unfold bstack; rewnb. fold ge. xomega.
+    - red. rewrite Pregmap.gss. inversion 1; subst.
+      repeat rewrite_stack_blocks. simpl. rewrite repr_stack_limit. unfold size_frame.
+      simpl. inversion 1. subst. simpl. omega.
+    - red. rewrite Pregmap.gss. inversion 1; subst.
+      rewrite repr_stack_limit. apply Mem.stack_limit_aligned.
+    - red. intros o k p.
+      repeat rewrite_perms. rewrite peq_true. intros (A & B).
+      generalize (Mem.stack_limit_range). trim B; auto. trim B ; auto. split; auto. omega.
+    - red; intros.
+      repeat rewrite_perms. rewrite peq_true. split; auto. intros; constructor.
+    - red.
+      repeat rewrite_stack_blocks. inversion 1; subst.
+      repeat econstructor.
+    - rewrite Pregmap.gss. eauto.
+    - red.
+      intros b delta o k p INJ. repeat rewrite_perms. destr. omega. intro P.
+      rewrite F'O in INJ by auto. unfold Mem.flat_inj in INJ.
+      revert INJ.
+      apply Mem.perm_valid_block in P. red in P; revert P.
+      rewnb. destr.
+    - repeat rewrite_stack_blocks.
+      inversion 1; subst.
+      repeat econstructor; eauto.
+      simpl. rewrite Z.max_r by omega. change (align 0 8) with 0. rewrite F'B. f_equal. f_equal. omega. simpl. rewrite Z.max_r ; intros;  omega.
+    - red. repeat rewrite_stack_blocks. inversion 1; subst. simpl.
+      intros. destruct H as [[]|[[A|[]]|[]]]. inv A.
+      simpl. rewrite Z.max_r by omega. change (align 0 8) with 0. omega.
+    - intros.
+      assert (Plt b (Genv.genv_next ge)).
+      {
+        unfold Genv.find_funct_ptr in H. repeat destr_in H.
+        eapply Genv.genv_defs_range in Heqo; eauto.
+      }
+      rewrite F'O. unfold Mem.flat_inj. rewnb. fold ge. destr. xomega.
+      apply Plt_ne; auto.
+    - intros.
+      assert (Plt b (Genv.genv_next ge)).
+      {
+        eapply Genv.genv_defs_range in H; eauto.
+      }
+      rewrite F'O. unfold Mem.flat_inj. rewnb. fold ge. destr. xomega.
+      apply Plt_ne; auto.
+    - split.
+      simpl; intros.
+      assert (Plt b (Genv.genv_next ge)).
+      {
+        eapply Genv.genv_symb_range in H; eauto.
+      }
+      rewrite F'O. unfold Mem.flat_inj. rewnb. fold ge. destr. xomega.
+      apply Plt_ne; auto.
+      intros b1 b2 delta FB. destruct (peq b1 bstack); subst.
+      rewrite F'B in FB; inv FB; auto.
+      rewrite F'O in FB; auto.
+      unfold Mem.flat_inj in FB; repeat destr_in FB; auto.
+    - rewnb. fold ge. xomega.
+    - rewnb. fold ge. xomega.
+    - repeat rewrite_stack_blocks. simpl. right; left; left. simpl. reflexivity.
+  Qed.
+
+  Lemma transf_final_states:
+    forall istk isp j o st1 st2 r,
+      match_states istk isp j o st1 st2 -> Asm.final_state st1 r -> final_state st2 r.
+  Proof.
+    inversion 1; subst.
+    inversion 1; subst.
+    econstructor.
+    generalize (RINJ PC). rewrite H3. unfold Vnullptr. destruct ptr64; inversion 1; auto.
+    generalize (RINJ RAX). rewrite H5. unfold Vnullptr. destruct ptr64; inversion 1; auto.
+  Qed.
+  
+  Theorem transf_program_correct:
+    asm_prog_no_rsp ge ->
+    forward_simulation (Asm.semantics
+                          prog
+                          ((Some (make_singleton_frame_adt (Genv.genv_next ge) 0 0), nil) :: nil))
+                       (RawAsm.semantics prog (Pregmap.init Vundef)).
+  Proof.
+    intros APNR.
+    eapply forward_simulation_step with (fun s1 s2 => exists j o, match_states _  (Genv.genv_next ge) j o s1 s2).
+    - simpl. reflexivity. 
+    - simpl. intros s1 IS; inversion IS.
+      exploit match_initial_states. eauto.
+      intros (s' & j & ostack & MS & MIS); eexists; split; eauto. inv MIS. eauto.
+    - simpl. intros s1 s2 r (j & o & MS) FS. eapply transf_final_states; eauto.
+    - simpl. intros s1 t s1' STEP s2 (j & o & MS). 
+      edestruct step_simulation as (isp' & j' & o' & STEP' & MS'); eauto.
+      reflexivity.
+  Qed.
+  
+End WITHMEMORYMODEL.
